@prefix :        <http://www.purl.org/i4go/variant-domain/productionplant#> .
@prefix owl:     <http://www.w3.org/2002/07/owl#> .
@prefix rdf:     <http://www.w3.org/1999/02/22-rdf-syntax-ns#> .
@prefix terms:   <http://purl.org/dc/terms/> .
@prefix ns:      <http://creativecommons.org/ns#> .
@prefix xsd:     <http://www.w3.org/2001/XMLSchema#> .
@prefix rdfs:    <http://www.w3.org/2000/01/rdf-schema#> .
@prefix dc:      <http://purl.org/dc/elements/1.1/> .

<http://www.w3id.org/ecsel-dr-SO#hasPlantName>
      a       owl:DatatypeProperty ;
      rdfs:comment "The name of the plant"@en ;
      rdfs:label "has plant name"@en ;
      rdfs:subPropertyOf owl:topDataProperty .

<http://www.w3id.org/ecsel-dr-SO#hasPlantInternal>
      a       owl:DatatypeProperty ;
      rdfs:comment "Does the plant belong to the company or to an external partner"@en ;
      rdfs:label "has plant internal"@en ;
      rdfs:subPropertyOf owl:topDataProperty .

<http://www.w3id.org/ecsel-dr-SO#Plant>
      a       owl:Class ;
      rdfs:comment "The “Plant” entity describes the plant as a physical location of one or more fabs. The Plant belongs to a supply chain and can either be internal or external. (master entity)"@en ;
      rdfs:label "Plant"@en ;
      rdfs:subClassOf <http://www.owl-ontologies.com/mason.owl#Resource> .

terms:issued
      a       owl:AnnotationProperty .

<http://www.purl.org/i4go/variant-domain/productionplant>
      a       owl:Ontology ;
      rdfs:comment "The 'Production Plant' ontology module represents data related to plant topology, including the concrete equipment of an actual project – the instance data."@en ;
      dc:title "Production Plant ontology"@en ;
      terms:creator """Javier Cuenca <mailto:jcuenca@mondragon.edu>
Felix Larrinaga <mailto:flarrinaga@mondragon.edu>"""@en ;
      terms:issued "2021-05-25"@en ;
      owl:imports <http://www.purl.org/i4go/variant-domain/manufacturingresource> ;
      owl:versionInfo "1.0"@en .

<http://www.w3id.org/ecsel-dr-SO#hasFab>
      a       owl:ObjectProperty ;
      rdfs:comment "This property is used to relate a production plant with the factory ot belongs to"@en ;
      rdfs:domain <http://www.w3id.org/ecsel-dr-SO#Plant> ;
      rdfs:label "has fab"@en ;
      rdfs:range <http://www.w3id.org/ecsel-dr-SO#Fab> ;
      rdfs:subPropertyOf owl:topObjectProperty .

terms:creator
      a       owl:AnnotationProperty .

dc:title
      a       owl:AnnotationProperty .

<http://www.w3id.org/ecsel-dr-SO#hasPlantID>
      a       owl:DatatypeProperty ;
      rdfs:comment "Will generally refer to the geographical location of the plant"@en ;
      rdfs:label "has plant ID"@en ;
      rdfs:subPropertyOf owl:topDataProperty .

ns:license
      a       owl:AnnotationProperty .

<http://www.w3id.org/ecsel-dr-SO#Fab>
      a       owl:Class ;
      rdfs:comment "The “Fab” entity depicts the fab as a technological and physical production unit. (master entity)"@en ;
      rdfs:label "Fab"@en ;
      rdfs:subClassOf <http://www.purl.org/i4go/variant-domain/manufacturingresource/GeographicResource> .
