_:AX2dX505cc3dcX3aX17a61a951eeX3aXX2dX7ff9 <http://www.w3.org/1999/02/22-rdf-syntax-ns#rest> <http://www.w3.org/1999/02/22-rdf-syntax-ns#nil> .
_:AX2dX505cc3dcX3aX17a61a951eeX3aXX2dX7ff9 <http://www.w3.org/1999/02/22-rdf-syntax-ns#first> <http://www.w3id.org/ecsel-dr-AH#System-of-Systems> .
<http://www.purl.org/i4go/variant-domain/service/DataFormat> <http://www.w3.org/2000/01/rdf-schema#label> "Data format"@en .
<http://www.purl.org/i4go/variant-domain/service/DataFormat> <http://www.w3.org/2000/01/rdf-schema#comment> "This class is used to represent any data format."@en .
<http://www.purl.org/i4go/variant-domain/service/DataFormat> <http://www.w3.org/1999/02/22-rdf-syntax-ns#type> <http://www.w3.org/2002/07/owl#Class> .
_:AX2dX505cc3dcX3aX17a61a951eeX3aXX2dX7ff3 <http://www.w3.org/2002/07/owl#maxCardinality> "1"^^<http://www.w3.org/2001/XMLSchema#nonNegativeInteger> .
_:AX2dX505cc3dcX3aX17a61a951eeX3aXX2dX7ff3 <http://www.w3.org/2002/07/owl#onProperty> <http://www.semanticweb.org/ontologies/2010/01/core-soa.owl#interactionAspect> .
_:AX2dX505cc3dcX3aX17a61a951eeX3aXX2dX7ff3 <http://www.w3.org/1999/02/22-rdf-syntax-ns#type> <http://www.w3.org/2002/07/owl#Restriction> .
<http://www.w3id.org/ecsel-dr-AH#isInformationModelOf> <http://www.w3.org/2000/01/rdf-schema#label> "is information model of"@en .
<http://www.w3id.org/ecsel-dr-AH#isInformationModelOf> <http://www.w3.org/2000/01/rdf-schema#subPropertyOf> <http://www.w3.org/2002/07/owl#topObjectProperty> .
<http://www.w3id.org/ecsel-dr-AH#isInformationModelOf> <http://www.w3.org/1999/02/22-rdf-syntax-ns#type> <http://www.w3.org/2002/07/owl#ObjectProperty> .
<http://www.w3id.org/ecsel-dr-AH#isServiceProducerOf> <http://www.w3.org/2000/01/rdf-schema#label> "is service producer of"@en .
<http://www.w3id.org/ecsel-dr-AH#isServiceProducerOf> <http://www.w3.org/2002/07/owl#inverseOf> <http://www.w3id.org/ecsel-dr-AH#producedBy> .
<http://www.w3id.org/ecsel-dr-AH#isServiceProducerOf> <http://www.w3.org/2000/01/rdf-schema#subPropertyOf> <http://www.w3.org/2002/07/owl#topObjectProperty> .
<http://www.w3id.org/ecsel-dr-AH#isServiceProducerOf> <http://www.w3.org/1999/02/22-rdf-syntax-ns#type> <http://www.w3.org/2002/07/owl#ObjectProperty> .
<http://www.semanticweb.org/ontologies/2010/01/core-soa.owl#isInterfaceOf> <http://www.w3.org/2000/01/rdf-schema#label> "is interface of"@en .
<http://www.semanticweb.org/ontologies/2010/01/core-soa.owl#isInterfaceOf> <http://www.w3.org/2000/01/rdf-schema#subPropertyOf> <http://www.w3.org/2002/07/owl#topObjectProperty> .
<http://www.semanticweb.org/ontologies/2010/01/core-soa.owl#isInterfaceOf> <http://www.w3.org/1999/02/22-rdf-syntax-ns#type> <http://www.w3.org/2002/07/owl#ObjectProperty> .
_:AX2dX505cc3dcX3aX17a61a951eeX3aXX2dX7ff8 <http://www.w3.org/2002/07/owl#minCardinality> "1"^^<http://www.w3.org/2001/XMLSchema#nonNegativeInteger> .
_:AX2dX505cc3dcX3aX17a61a951eeX3aXX2dX7ff8 <http://www.w3.org/2002/07/owl#onProperty> <http://www.semanticweb.org/ontologies/2010/01/core-soa.owl#hasInterface> .
_:AX2dX505cc3dcX3aX17a61a951eeX3aXX2dX7ff8 <http://www.w3.org/1999/02/22-rdf-syntax-ns#type> <http://www.w3.org/2002/07/owl#Restriction> .
<http://www.purl.org/i4go/variant-domain/service/TransferProtocol> <http://www.w3.org/2000/01/rdf-schema#label> "Transfer protocol"@en .
<http://www.purl.org/i4go/variant-domain/service/TransferProtocol> <http://www.w3.org/2000/01/rdf-schema#comment> "This class is used to reptresent a data transfer protocol."@en .
<http://www.purl.org/i4go/variant-domain/service/TransferProtocol> <http://www.w3.org/2000/01/rdf-schema#subClassOf> <http://www.purl.org/i4go/variant-domain/service/CommunicationTechnology> .
<http://www.purl.org/i4go/variant-domain/service/TransferProtocol> <http://www.w3.org/1999/02/22-rdf-syntax-ns#type> <http://www.w3.org/2002/07/owl#Class> .
_:AX2dX505cc3dcX3aX17a61a951eeX3aXX2dX7ff2 <http://www.w3.org/2002/07/owl#maxCardinality> "1"^^<http://www.w3.org/2001/XMLSchema#nonNegativeInteger> .
_:AX2dX505cc3dcX3aX17a61a951eeX3aXX2dX7ff2 <http://www.w3.org/2002/07/owl#onProperty> <http://www.semanticweb.org/ontologies/2010/01/core-soa.owl#legalAspect> .
_:AX2dX505cc3dcX3aX17a61a951eeX3aXX2dX7ff2 <http://www.w3.org/1999/02/22-rdf-syntax-ns#type> <http://www.w3.org/2002/07/owl#Restriction> .
<http://www.w3id.org/ecsel-dr-AH#hasInformationModel> <http://www.w3.org/2000/01/rdf-schema#label> "has information model"@en .
<http://www.w3id.org/ecsel-dr-AH#hasInformationModel> <http://www.w3.org/2000/01/rdf-schema#comment> "This property is used to relate services with their information model."@en .
<http://www.w3id.org/ecsel-dr-AH#hasInformationModel> <http://www.w3.org/2000/01/rdf-schema#range> <http://www.w3id.org/ecsel-dr-AH#InformationModel> .
<http://www.w3id.org/ecsel-dr-AH#hasInformationModel> <http://www.w3.org/2000/01/rdf-schema#domain> <http://purl.org/dc/dcmitype/Service> .
<http://www.w3id.org/ecsel-dr-AH#hasInformationModel> <http://www.w3.org/2002/07/owl#inverseOf> <http://www.w3id.org/ecsel-dr-AH#isInformationModelOf> .
<http://www.w3id.org/ecsel-dr-AH#hasInformationModel> <http://www.w3.org/2000/01/rdf-schema#subPropertyOf> <http://www.w3.org/2002/07/owl#topObjectProperty> .
<http://www.w3id.org/ecsel-dr-AH#hasInformationModel> <http://www.w3.org/1999/02/22-rdf-syntax-ns#type> <http://www.w3.org/2002/07/owl#ObjectProperty> .
<http://www.semanticweb.org/ontologies/2010/01/core-soa.owl#interactionAspect> <http://www.w3.org/2000/01/rdf-schema#label> "interfaction aspect"@en .
<http://www.semanticweb.org/ontologies/2010/01/core-soa.owl#interactionAspect> <http://www.w3.org/2000/01/rdf-schema#domain> <http://www.semanticweb.org/ontologies/2010/01/core-soa.owl#ServiceContract> .
<http://www.semanticweb.org/ontologies/2010/01/core-soa.owl#interactionAspect> <http://www.w3.org/2000/01/rdf-schema#subPropertyOf> <http://www.w3.org/2002/07/owl#topDataProperty> .
<http://www.semanticweb.org/ontologies/2010/01/core-soa.owl#interactionAspect> <http://www.w3.org/1999/02/22-rdf-syntax-ns#type> <http://www.w3.org/2002/07/owl#DatatypeProperty> .
<http://www.w3id.org/ecsel-dr-AH#producedBy> <http://www.w3.org/2000/01/rdf-schema#label> "produced by"@en .
<http://www.w3id.org/ecsel-dr-AH#producedBy> <http://www.w3.org/2000/01/rdf-schema#comment> "This property relates the servicies with the software systems that provide them."@en .
<http://www.w3id.org/ecsel-dr-AH#producedBy> <http://www.w3.org/2000/01/rdf-schema#range> <http://purl.org/dc/dcmitype/Software> .
<http://www.w3id.org/ecsel-dr-AH#producedBy> <http://www.w3.org/2000/01/rdf-schema#domain> <http://purl.org/dc/dcmitype/Service> .
<http://www.w3id.org/ecsel-dr-AH#producedBy> <http://www.w3.org/2002/07/owl#inverseOf> <http://www.w3id.org/ecsel-dr-AH#produces> .
<http://www.w3id.org/ecsel-dr-AH#producedBy> <http://www.w3.org/2000/01/rdf-schema#subPropertyOf> <http://www.w3.org/2002/07/owl#topObjectProperty> .
<http://www.w3id.org/ecsel-dr-AH#producedBy> <http://www.w3.org/1999/02/22-rdf-syntax-ns#type> <http://www.w3.org/2002/07/owl#ObjectProperty> .
<http://www.semanticweb.org/ontologies/2010/01/core-soa.owl#constraints> <http://www.w3.org/2000/01/rdf-schema#label> "constraints"@en .
<http://www.semanticweb.org/ontologies/2010/01/core-soa.owl#constraints> <http://www.w3.org/2000/01/rdf-schema#domain> <http://www.semanticweb.org/ontologies/2010/01/core-soa.owl#ServiceInterface> .
<http://www.semanticweb.org/ontologies/2010/01/core-soa.owl#constraints> <http://www.w3.org/2000/01/rdf-schema#subPropertyOf> <http://www.w3.org/2002/07/owl#topDataProperty> .
<http://www.semanticweb.org/ontologies/2010/01/core-soa.owl#constraints> <http://www.w3.org/1999/02/22-rdf-syntax-ns#type> <http://www.w3.org/2002/07/owl#DatatypeProperty> .
_:AX2dX505cc3dcX3aX17a61a951eeX3aXX2dX7ff7 <http://www.w3.org/2002/07/owl#minCardinality> "1"^^<http://www.w3.org/2001/XMLSchema#nonNegativeInteger> .
_:AX2dX505cc3dcX3aX17a61a951eeX3aXX2dX7ff7 <http://www.w3.org/2002/07/owl#onProperty> <http://www.semanticweb.org/ontologies/2010/01/core-soa.owl#isContractFor> .
_:AX2dX505cc3dcX3aX17a61a951eeX3aXX2dX7ff7 <http://www.w3.org/1999/02/22-rdf-syntax-ns#type> <http://www.w3.org/2002/07/owl#Restriction> .
<http://purl.org/ontology/is/core#InfoService> <http://www.w3.org/2000/01/rdf-schema#label> "Info service"@en .
<http://purl.org/ontology/is/core#InfoService> <http://www.w3.org/2000/01/rdf-schema#comment> "Service offered by a system that provides information"@en .
<http://purl.org/ontology/is/core#InfoService> <http://www.w3.org/2000/01/rdf-schema#subClassOf> <http://purl.org/dc/dcmitype/Service> .
<http://purl.org/ontology/is/core#InfoService> <http://www.w3.org/1999/02/22-rdf-syntax-ns#type> <http://www.w3.org/2002/07/owl#Class> .
<http://www.semanticweb.org/ontologies/2010/01/core-soa.owl#isSpecifiedBy> <http://www.w3.org/2000/01/rdf-schema#label> "is specified by"@en .
<http://www.semanticweb.org/ontologies/2010/01/core-soa.owl#isSpecifiedBy> <http://www.w3.org/2000/01/rdf-schema#subPropertyOf> <http://www.w3.org/2002/07/owl#topObjectProperty> .
<http://www.semanticweb.org/ontologies/2010/01/core-soa.owl#isSpecifiedBy> <http://www.w3.org/1999/02/22-rdf-syntax-ns#type> <http://www.w3.org/2002/07/owl#ObjectProperty> .
<http://purl.org/dc/dcmitype/Service> <http://www.w3.org/2000/01/rdf-schema#label> "Service"@en .
<http://purl.org/dc/dcmitype/Service> <http://www.w3.org/2000/01/rdf-schema#comment> "Distinct part of the functionality that is provided by an entity through interfaces"@en .
<http://purl.org/dc/dcmitype/Service> <http://www.w3.org/2000/01/rdf-schema#subClassOf> _:AX2dX505cc3dcX3aX17a61a951eeX3aXX2dX7ff8 .
<http://purl.org/dc/dcmitype/Service> <http://www.w3.org/1999/02/22-rdf-syntax-ns#type> <http://www.w3.org/2002/07/owl#Class> .
<http://www.w3id.org/ecsel-dr-AH#isDocumentedBy> <http://www.w3.org/2000/01/rdf-schema#label> "is documented by"@en .
<http://www.w3id.org/ecsel-dr-AH#isDocumentedBy> <http://www.w3.org/2000/01/rdf-schema#comment> "This property is used to relate systems and services with their documentation"@en .
<http://www.w3id.org/ecsel-dr-AH#isDocumentedBy> <http://www.w3.org/2000/01/rdf-schema#range> <http://www.purl.org/i4go/variant-domain/service/ServiceDocumentation> .
<http://www.w3id.org/ecsel-dr-AH#isDocumentedBy> <http://www.w3.org/2000/01/rdf-schema#range> <http://www.purl.org/i4go/common-domain/system/SystemDocumentation> .
<http://www.w3id.org/ecsel-dr-AH#isDocumentedBy> <http://www.w3.org/2000/01/rdf-schema#domain> _:AX2dX505cc3dcX3aX17a61a951eeX3aXX2dX7ffc .
<http://www.w3id.org/ecsel-dr-AH#isDocumentedBy> <http://www.w3.org/2000/01/rdf-schema#subPropertyOf> <http://www.w3.org/2002/07/owl#topObjectProperty> .
<http://www.w3id.org/ecsel-dr-AH#isDocumentedBy> <http://www.w3.org/1999/02/22-rdf-syntax-ns#type> <http://www.w3.org/2002/07/owl#ObjectProperty> .
<http://www.w3id.org/ecsel-dr-AH#usesTransferProtocol> <http://www.w3.org/2000/01/rdf-schema#label> "uses transfer protocol"@en .
<http://www.w3id.org/ecsel-dr-AH#usesTransferProtocol> <http://www.w3.org/2000/01/rdf-schema#comment> "This property is used to relate a service with the data transfer protocol it uses."@en .
<http://www.w3id.org/ecsel-dr-AH#usesTransferProtocol> <http://www.w3.org/2000/01/rdf-schema#subPropertyOf> <http://www.w3id.org/ecsel-dr-AH#usesCommTech> .
<http://www.w3id.org/ecsel-dr-AH#usesTransferProtocol> <http://www.w3.org/1999/02/22-rdf-syntax-ns#type> <http://www.w3.org/2002/07/owl#ObjectProperty> .
<http://www.w3id.org/ecsel-dr-AH#InformationModel> <http://www.w3.org/2000/01/rdf-schema#label> "Information model"@en .
<http://www.w3id.org/ecsel-dr-AH#InformationModel> <http://www.w3.org/2000/01/rdf-schema#comment> "An information model in software engineering is a representation of concepts and the relationships, constraints, rules, and operations to specify data semantics for a chosen domain of discourse."@en .
<http://www.w3id.org/ecsel-dr-AH#InformationModel> <http://www.w3.org/1999/02/22-rdf-syntax-ns#type> <http://www.w3.org/2002/07/owl#Class> .
_:AX2dX505cc3dcX3aX17a61a951eeX3aXX2dX7ff1 <http://www.w3.org/2002/07/owl#minCardinality> "1"^^<http://www.w3.org/2001/XMLSchema#nonNegativeInteger> .
_:AX2dX505cc3dcX3aX17a61a951eeX3aXX2dX7ff1 <http://www.w3.org/2002/07/owl#onProperty> <http://www.semanticweb.org/ontologies/2010/01/core-soa.owl#constraints> .
_:AX2dX505cc3dcX3aX17a61a951eeX3aXX2dX7ff1 <http://www.w3.org/1999/02/22-rdf-syntax-ns#type> <http://www.w3.org/2002/07/owl#Restriction> .
<http://www.purl.org/i4go/variant-domain/service/Point-to-PointCommunicationTechnology> <http://www.w3.org/2000/01/rdf-schema#label> "Point-to-point communication technology"@en .
<http://www.purl.org/i4go/variant-domain/service/Point-to-PointCommunicationTechnology> <http://www.w3.org/2000/01/rdf-schema#comment> "In telecommunications, a point-to-point connection refers to a communications connection between two communication endpoints or nodes. An example is a telephone call, in which one telephone is connected with one other, and what is said by one caller can only be heard by the other."@en .
<http://www.purl.org/i4go/variant-domain/service/Point-to-PointCommunicationTechnology> <http://www.w3.org/2000/01/rdf-schema#subClassOf> <http://www.purl.org/i4go/variant-domain/service/CommunicationTechnology> .
<http://www.purl.org/i4go/variant-domain/service/Point-to-PointCommunicationTechnology> <http://www.w3.org/1999/02/22-rdf-syntax-ns#type> <http://www.w3.org/2002/07/owl#Class> .
<http://www.purl.org/i4go/variant-domain/service/End-to-EndCommunicationTechnology> <http://www.w3.org/2000/01/rdf-schema#label> "End-to-end communication technology"@en .
<http://www.purl.org/i4go/variant-domain/service/End-to-EndCommunicationTechnology> <http://www.w3.org/2000/01/rdf-schema#comment> "The end-to-end principle is a network design method in which application-specific features are kept at communication end points."@en .
<http://www.purl.org/i4go/variant-domain/service/End-to-EndCommunicationTechnology> <http://www.w3.org/2000/01/rdf-schema#subClassOf> <http://www.purl.org/i4go/variant-domain/service/CommunicationTechnology> .
<http://www.purl.org/i4go/variant-domain/service/End-to-EndCommunicationTechnology> <http://www.w3.org/1999/02/22-rdf-syntax-ns#type> <http://www.w3.org/2002/07/owl#Class> .
<http://www.semanticweb.org/ontologies/2010/01/core-soa.owl#hasInterface> <http://www.w3.org/2000/01/rdf-schema#label> "has interface"@en .
<http://www.semanticweb.org/ontologies/2010/01/core-soa.owl#hasInterface> <http://www.w3.org/2000/01/rdf-schema#comment> "This property is used to relate the servicies with their interfaces"@en .
<http://www.semanticweb.org/ontologies/2010/01/core-soa.owl#hasInterface> <http://www.w3.org/2002/07/owl#inverseOf> <http://www.semanticweb.org/ontologies/2010/01/core-soa.owl#isInterfaceOf> .
<http://www.semanticweb.org/ontologies/2010/01/core-soa.owl#hasInterface> <http://www.w3.org/2000/01/rdf-schema#subPropertyOf> <http://www.w3.org/2002/07/owl#topObjectProperty> .
<http://www.semanticweb.org/ontologies/2010/01/core-soa.owl#hasInterface> <http://www.w3.org/1999/02/22-rdf-syntax-ns#type> <http://www.w3.org/2002/07/owl#ObjectProperty> .
<http://www.purl.org/i4go/variant-domain/service/CommunicationSecurityMechanism> <http://www.w3.org/2000/01/rdf-schema#label> "Communication technology mecanism"@en .
<http://www.purl.org/i4go/variant-domain/service/CommunicationSecurityMechanism> <http://www.w3.org/2000/01/rdf-schema#comment> "Corresponds to a part of OSI layer 5"@en .
<http://www.purl.org/i4go/variant-domain/service/CommunicationSecurityMechanism> <http://www.w3.org/2000/01/rdf-schema#subClassOf> <http://www.purl.org/i4go/variant-domain/service/CommunicationTechnology> .
<http://www.purl.org/i4go/variant-domain/service/CommunicationSecurityMechanism> <http://www.w3.org/1999/02/22-rdf-syntax-ns#type> <http://www.w3.org/2002/07/owl#Class> .
<http://www.w3id.org/ecsel-dr-AH#hasMethod> <http://www.w3.org/2000/01/rdf-schema#label> "has method"@en .
<http://www.w3id.org/ecsel-dr-AH#hasMethod> <http://www.w3.org/2000/01/rdf-schema#comment> "This property is used to relate servicies with the methods they provide."@en .
<http://www.w3id.org/ecsel-dr-AH#hasMethod> <http://www.w3.org/2002/07/owl#inverseOf> <http://www.w3id.org/ecsel-dr-AH#isMethodOf> .
<http://www.w3id.org/ecsel-dr-AH#hasMethod> <http://www.w3.org/2000/01/rdf-schema#subPropertyOf> <http://www.w3.org/2002/07/owl#topObjectProperty> .
<http://www.w3id.org/ecsel-dr-AH#hasMethod> <http://www.w3.org/1999/02/22-rdf-syntax-ns#type> <http://www.w3.org/2002/07/owl#ObjectProperty> .
<http://www.semanticweb.org/ontologies/2010/01/core-soa.owl#ServiceInterface> <http://www.w3.org/2000/01/rdf-schema#label> "Service interface"@en .
<http://www.semanticweb.org/ontologies/2010/01/core-soa.owl#ServiceInterface> <http://www.w3.org/2000/01/rdf-schema#comment> "A service interface is a published interface used to invoke a service. An interface can be implemented using any number of technologies, including WSDL, XML-RPC, COM+, CORBA (IDL), Java RMI, and others. A service interface can be described using multiple methods."@en .
<http://www.semanticweb.org/ontologies/2010/01/core-soa.owl#ServiceInterface> <http://www.w3.org/2000/01/rdf-schema#subClassOf> _:AX2dX505cc3dcX3aX17a61a951eeX3aXX2dX7ff0 .
<http://www.semanticweb.org/ontologies/2010/01/core-soa.owl#ServiceInterface> <http://www.w3.org/2000/01/rdf-schema#subClassOf> _:AX2dX505cc3dcX3aX17a61a951eeX3aXX2dX7ff1 .
<http://www.semanticweb.org/ontologies/2010/01/core-soa.owl#ServiceInterface> <http://www.w3.org/1999/02/22-rdf-syntax-ns#type> <http://www.w3.org/2002/07/owl#Class> .
_:AX2dX505cc3dcX3aX17a61a951eeX3aXX2dX7ff6 <http://www.w3.org/2002/07/owl#minCardinality> "1"^^<http://www.w3.org/2001/XMLSchema#nonNegativeInteger> .
_:AX2dX505cc3dcX3aX17a61a951eeX3aXX2dX7ff6 <http://www.w3.org/2002/07/owl#onProperty> <http://www.semanticweb.org/ontologies/2010/01/core-soa.owl#specifies> .
_:AX2dX505cc3dcX3aX17a61a951eeX3aXX2dX7ff6 <http://www.w3.org/1999/02/22-rdf-syntax-ns#type> <http://www.w3.org/2002/07/owl#Restriction> .
<http://www.semanticweb.org/ontologies/2010/01/core-soa.owl#ServiceContract> <http://www.w3.org/2000/01/rdf-schema#label> "Service contract"@en .
<http://www.semanticweb.org/ontologies/2010/01/core-soa.owl#ServiceContract> <http://www.w3.org/2000/01/rdf-schema#comment> "Is a document that sets out the provision and delivery of software services to customers through the internet."@en .
<http://www.semanticweb.org/ontologies/2010/01/core-soa.owl#ServiceContract> <http://www.w3.org/2000/01/rdf-schema#subClassOf> _:AX2dX505cc3dcX3aX17a61a951eeX3aXX2dX7ff2 .
<http://www.semanticweb.org/ontologies/2010/01/core-soa.owl#ServiceContract> <http://www.w3.org/2000/01/rdf-schema#subClassOf> _:AX2dX505cc3dcX3aX17a61a951eeX3aXX2dX7ff3 .
<http://www.semanticweb.org/ontologies/2010/01/core-soa.owl#ServiceContract> <http://www.w3.org/2000/01/rdf-schema#subClassOf> _:AX2dX505cc3dcX3aX17a61a951eeX3aXX2dX7ff4 .
<http://www.semanticweb.org/ontologies/2010/01/core-soa.owl#ServiceContract> <http://www.w3.org/2000/01/rdf-schema#subClassOf> _:AX2dX505cc3dcX3aX17a61a951eeX3aXX2dX7ff5 .
<http://www.semanticweb.org/ontologies/2010/01/core-soa.owl#ServiceContract> <http://www.w3.org/2000/01/rdf-schema#subClassOf> _:AX2dX505cc3dcX3aX17a61a951eeX3aXX2dX7ff6 .
<http://www.semanticweb.org/ontologies/2010/01/core-soa.owl#ServiceContract> <http://www.w3.org/2000/01/rdf-schema#subClassOf> _:AX2dX505cc3dcX3aX17a61a951eeX3aXX2dX7ff7 .
<http://www.semanticweb.org/ontologies/2010/01/core-soa.owl#ServiceContract> <http://www.w3.org/1999/02/22-rdf-syntax-ns#type> <http://www.w3.org/2002/07/owl#Class> .
<http://www.semanticweb.org/ontologies/2010/01/core-soa.owl#hasContract> <http://www.w3.org/2000/01/rdf-schema#label> "has contract"@en .
<http://www.semanticweb.org/ontologies/2010/01/core-soa.owl#hasContract> <http://www.w3.org/2000/01/rdf-schema#comment> "This property is used to relate a service with its service contract."@en .
<http://www.semanticweb.org/ontologies/2010/01/core-soa.owl#hasContract> <http://www.w3.org/2002/07/owl#inverseOf> <http://www.semanticweb.org/ontologies/2010/01/core-soa.owl#isContractFor> .
<http://www.semanticweb.org/ontologies/2010/01/core-soa.owl#hasContract> <http://www.w3.org/2000/01/rdf-schema#subPropertyOf> <http://www.w3.org/2002/07/owl#topObjectProperty> .
<http://www.semanticweb.org/ontologies/2010/01/core-soa.owl#hasContract> <http://www.w3.org/1999/02/22-rdf-syntax-ns#type> <http://www.w3.org/2002/07/owl#ObjectProperty> .
<http://www.semanticweb.org/ontologies/2010/01/core-soa.owl#Effect> <http://www.w3.org/2000/01/rdf-schema#label> "Effect"@en .
<http://www.semanticweb.org/ontologies/2010/01/core-soa.owl#Effect> <http://www.w3.org/2000/01/rdf-schema#comment> "The effect of a service contract."@en .
<http://www.semanticweb.org/ontologies/2010/01/core-soa.owl#Effect> <http://www.w3.org/1999/02/22-rdf-syntax-ns#type> <http://www.w3.org/2002/07/owl#Class> .
_:AX2dX505cc3dcX3aX17a61a951eeX3aXX2dX7ff0 <http://www.w3.org/2002/07/owl#maxCardinality> "1"^^<http://www.w3.org/2001/XMLSchema#nonNegativeInteger> .
_:AX2dX505cc3dcX3aX17a61a951eeX3aXX2dX7ff0 <http://www.w3.org/2002/07/owl#onProperty> <http://www.semanticweb.org/ontologies/2010/01/core-soa.owl#constraints> .
_:AX2dX505cc3dcX3aX17a61a951eeX3aXX2dX7ff0 <http://www.w3.org/1999/02/22-rdf-syntax-ns#type> <http://www.w3.org/2002/07/owl#Restriction> .
_:AX2dX505cc3dcX3aX17a61a951eeX3aXX2dX7ffc <http://www.w3.org/2002/07/owl#unionOf> _:AX2dX505cc3dcX3aX17a61a951eeX3aXX2dX7ffb .
_:AX2dX505cc3dcX3aX17a61a951eeX3aXX2dX7ffc <http://www.w3.org/1999/02/22-rdf-syntax-ns#type> <http://www.w3.org/2002/07/owl#Class> .
<http://www.w3id.org/ecsel-dr-PMV#OtherServices> <http://www.w3.org/2000/01/rdf-schema#label> "Other services"@en .
<http://www.w3id.org/ecsel-dr-PMV#OtherServices> <http://www.w3.org/2000/01/rdf-schema#comment> "Collection of other services used as input to a production process or which are created during a production process."@en .
<http://www.w3id.org/ecsel-dr-PMV#OtherServices> <http://www.w3.org/2000/01/rdf-schema#subClassOf> <http://purl.org/dc/dcmitype/Service> .
<http://www.w3id.org/ecsel-dr-PMV#OtherServices> <http://www.w3.org/1999/02/22-rdf-syntax-ns#type> <http://www.w3.org/2002/07/owl#Class> .
<http://www.w3.org/2002/07/owl#topObjectProperty> <http://www.w3.org/2000/01/rdf-schema#range> <http://www.w3id.org/ecsel-dr-AH#Method> .
<http://www.w3.org/2002/07/owl#topObjectProperty> <http://www.w3.org/2000/01/rdf-schema#domain> <http://purl.org/dc/dcmitype/Service> .
<http://www.w3id.org/ecsel-dr-AH#Method> <http://www.w3.org/2000/01/rdf-schema#label> "Method"@en .
<http://www.w3id.org/ecsel-dr-AH#Method> <http://www.w3.org/2000/01/rdf-schema#comment> "Method of a service: method that is provided by a service within a SoA."@en .
<http://www.w3id.org/ecsel-dr-AH#Method> <http://www.w3.org/1999/02/22-rdf-syntax-ns#type> <http://www.w3.org/2002/07/owl#Class> .
_:AX2dX505cc3dcX3aX17a61a951eeX3aXX2dX7ff5 <http://www.w3.org/2002/07/owl#minCardinality> "1"^^<http://www.w3.org/2001/XMLSchema#nonNegativeInteger> .
_:AX2dX505cc3dcX3aX17a61a951eeX3aXX2dX7ff5 <http://www.w3.org/2002/07/owl#onProperty> <http://www.semanticweb.org/ontologies/2010/01/core-soa.owl#interactionAspect> .
_:AX2dX505cc3dcX3aX17a61a951eeX3aXX2dX7ff5 <http://www.w3.org/1999/02/22-rdf-syntax-ns#type> <http://www.w3.org/2002/07/owl#Restriction> .
<http://www.semanticweb.org/ontologies/2010/01/core-soa.owl#isContractFor> <http://www.w3.org/2000/01/rdf-schema#label> "is contract for"@en .
<http://www.semanticweb.org/ontologies/2010/01/core-soa.owl#isContractFor> <http://www.w3.org/2000/01/rdf-schema#subPropertyOf> <http://www.w3.org/2002/07/owl#topObjectProperty> .
<http://www.semanticweb.org/ontologies/2010/01/core-soa.owl#isContractFor> <http://www.w3.org/1999/02/22-rdf-syntax-ns#type> <http://www.w3.org/2002/07/owl#ObjectProperty> .
<http://www.purl.org/i4go/variant-domain/service/CommunicationTechnology> <http://www.w3.org/2000/01/rdf-schema#label> "Communication technology"@en .
<http://www.purl.org/i4go/variant-domain/service/CommunicationTechnology> <http://www.w3.org/2000/01/rdf-schema#comment> "The communication technology used by a service."@en .
<http://www.purl.org/i4go/variant-domain/service/CommunicationTechnology> <http://www.w3.org/1999/02/22-rdf-syntax-ns#type> <http://www.w3.org/2002/07/owl#Class> .
<http://www.purl.org/i4go/variant-domain/service/ServiceDocumentation> <http://www.w3.org/2000/01/rdf-schema#label> "Service documentation"@en .
<http://www.purl.org/i4go/variant-domain/service/ServiceDocumentation> <http://www.w3.org/2000/01/rdf-schema#comment> "Collection of documents that contain the information about a service."@en .
<http://www.purl.org/i4go/variant-domain/service/ServiceDocumentation> <http://www.w3.org/1999/02/22-rdf-syntax-ns#type> <http://www.w3.org/2002/07/owl#Class> .
<http://www.w3id.org/ecsel-dr-AH#usesCommTech> <http://www.w3.org/2000/01/rdf-schema#label> "uses communication technology"@en .
<http://www.w3id.org/ecsel-dr-AH#usesCommTech> <http://www.w3.org/2000/01/rdf-schema#comment> "This property is used to relate a service with the communication technology it uses."@en .
<http://www.w3id.org/ecsel-dr-AH#usesCommTech> <http://www.w3.org/2000/01/rdf-schema#range> <http://www.purl.org/i4go/variant-domain/service/CommunicationTechnology> .
<http://www.w3id.org/ecsel-dr-AH#usesCommTech> <http://www.w3.org/2000/01/rdf-schema#domain> <http://purl.org/dc/dcmitype/Service> .
<http://www.w3id.org/ecsel-dr-AH#usesCommTech> <http://www.w3.org/2000/01/rdf-schema#subPropertyOf> <http://www.w3.org/2002/07/owl#topObjectProperty> .
<http://www.w3id.org/ecsel-dr-AH#usesCommTech> <http://www.w3.org/1999/02/22-rdf-syntax-ns#type> <http://www.w3.org/2002/07/owl#ObjectProperty> .
<http://www.w3id.org/ecsel-dr-AH#usesSecurityMechanism> <http://www.w3.org/2000/01/rdf-schema#label> "uses security mechanism"@en .
<http://www.w3id.org/ecsel-dr-AH#usesSecurityMechanism> <http://www.w3.org/2000/01/rdf-schema#comment> "This property is used to relate a service with the security mechanism it uses."@en .
<http://www.w3id.org/ecsel-dr-AH#usesSecurityMechanism> <http://www.w3.org/2000/01/rdf-schema#range> <http://www.purl.org/i4go/variant-domain/service/CommunicationSecurityMechanism> .
<http://www.w3id.org/ecsel-dr-AH#usesSecurityMechanism> <http://www.w3.org/2000/01/rdf-schema#domain> <http://purl.org/dc/dcmitype/Service> .
<http://www.w3id.org/ecsel-dr-AH#usesSecurityMechanism> <http://www.w3.org/2000/01/rdf-schema#subPropertyOf> <http://www.w3id.org/ecsel-dr-AH#usesCommTech> .
<http://www.w3id.org/ecsel-dr-AH#usesSecurityMechanism> <http://www.w3.org/1999/02/22-rdf-syntax-ns#type> <http://www.w3.org/2002/07/owl#ObjectProperty> .
_:AX2dX505cc3dcX3aX17a61a951eeX3aXX2dX7ffb <http://www.w3.org/1999/02/22-rdf-syntax-ns#rest> _:AX2dX505cc3dcX3aX17a61a951eeX3aXX2dX7ffa .
_:AX2dX505cc3dcX3aX17a61a951eeX3aXX2dX7ffb <http://www.w3.org/1999/02/22-rdf-syntax-ns#first> <http://purl.org/dc/dcmitype/Service> .
<http://www.semanticweb.org/ontologies/2010/01/core-soa.owl#legalAspect> <http://www.w3.org/2000/01/rdf-schema#label> "legal aspect"@en .
<http://www.semanticweb.org/ontologies/2010/01/core-soa.owl#legalAspect> <http://www.w3.org/2000/01/rdf-schema#domain> <http://www.semanticweb.org/ontologies/2010/01/core-soa.owl#ServiceContract> .
<http://www.semanticweb.org/ontologies/2010/01/core-soa.owl#legalAspect> <http://www.w3.org/2000/01/rdf-schema#subPropertyOf> <http://www.w3.org/2002/07/owl#topDataProperty> .
<http://www.semanticweb.org/ontologies/2010/01/core-soa.owl#legalAspect> <http://www.w3.org/1999/02/22-rdf-syntax-ns#type> <http://www.w3.org/2002/07/owl#DatatypeProperty> .
<http://www.semanticweb.org/ontologies/2010/01/core-soa.owl#specifies> <http://www.w3.org/2000/01/rdf-schema#label> "specifies"@en .
<http://www.semanticweb.org/ontologies/2010/01/core-soa.owl#specifies> <http://www.w3.org/2000/01/rdf-schema#comment> "This property relates a service contract with the effect it specifies."@en .
<http://www.semanticweb.org/ontologies/2010/01/core-soa.owl#specifies> <http://www.w3.org/2000/01/rdf-schema#subPropertyOf> <http://www.w3.org/2002/07/owl#topObjectProperty> .
<http://www.semanticweb.org/ontologies/2010/01/core-soa.owl#specifies> <http://www.w3.org/1999/02/22-rdf-syntax-ns#type> <http://www.w3.org/2002/07/owl#ObjectProperty> .
<http://www.w3id.org/ecsel-dr-AH#isMethodOf> <http://www.w3.org/2000/01/rdf-schema#label> "is method of"@en .
<http://www.w3id.org/ecsel-dr-AH#isMethodOf> <http://www.w3.org/2000/01/rdf-schema#subPropertyOf> <http://www.w3.org/2002/07/owl#topObjectProperty> .
<http://www.w3id.org/ecsel-dr-AH#isMethodOf> <http://www.w3.org/1999/02/22-rdf-syntax-ns#type> <http://www.w3.org/2002/07/owl#ObjectProperty> .
<http://www.purl.org/i4go/variant-domain/service/DataLinkAndMediaAccessTechnology> <http://www.w3.org/2000/01/rdf-schema#label> "Data link and media access technology"@en .
<http://www.purl.org/i4go/variant-domain/service/DataLinkAndMediaAccessTechnology> <http://www.w3.org/2000/01/rdf-schema#comment> "Corresponds to OSI layer 1 and 2 technologies, like Ethernet, WLAN (802.11), WPAN (802.15.4), EtherCAT, ProfiNet, ..."@en .
<http://www.purl.org/i4go/variant-domain/service/DataLinkAndMediaAccessTechnology> <http://www.w3.org/2000/01/rdf-schema#subClassOf> <http://www.purl.org/i4go/variant-domain/service/CommunicationTechnology> .
<http://www.purl.org/i4go/variant-domain/service/DataLinkAndMediaAccessTechnology> <http://www.w3.org/1999/02/22-rdf-syntax-ns#type> <http://www.w3.org/2002/07/owl#Class> .
<http://www.purl.org/i4go/variant-domain/service> <http://creativecommons.org/ns#license> "https://creativecommons.org/licenses/by-nc/4.0/"@en .
<http://www.purl.org/i4go/variant-domain/service> <http://purl.org/dc/terms/issued> "20201-05-04"@en .
<http://www.purl.org/i4go/variant-domain/service> <http://purl.org/dc/elements/1.1/title> "Service ontology"@en .
<http://www.purl.org/i4go/variant-domain/service> <http://purl.org/dc/terms/creator> "Javier Cuenca <mailto:jcuenca@mondragon.edu>\nFelix Larrinaga <mailto:flarrinaga@mondragon.edu>"@en .
<http://www.purl.org/i4go/variant-domain/service> <http://www.w3.org/2002/07/owl#versionInfo> "1.0"@en .
<http://www.purl.org/i4go/variant-domain/service> <http://www.w3.org/2000/01/rdf-schema#comment> "The 'Service' ontology module represents the data about the functionalities provided by devices."@en .
<http://www.purl.org/i4go/variant-domain/service> <http://www.w3.org/2002/07/owl#imports> <http://www.purl.org/i4go/variant-domain/software> .
<http://www.purl.org/i4go/variant-domain/service> <http://www.w3.org/1999/02/22-rdf-syntax-ns#type> <http://www.w3.org/2002/07/owl#Ontology> .
<http://www.w3id.org/ecsel-dr-AH#produces> <http://www.w3.org/2000/01/rdf-schema#label> "produces"@en .
<http://www.w3id.org/ecsel-dr-AH#produces> <http://www.w3.org/2000/01/rdf-schema#comment> "Relation expressing that a software system produces a service. \nEquivalent names for this relation include\n- offers\n- provides \n- isServiceProducerOf \nSince Arrowhead uses the pair produce / consume and corresponding service producer / service consumer adressing the relations and the software systems, this ontology uses these names for the relations too. \nIf it is needed, object properties with other names can be added and stated to be equivalent to these ones."@en .
<http://www.w3id.org/ecsel-dr-AH#produces> <http://www.w3.org/2000/01/rdf-schema#subPropertyOf> <http://www.w3.org/2002/07/owl#topObjectProperty> .
<http://www.w3id.org/ecsel-dr-AH#produces> <http://www.w3.org/1999/02/22-rdf-syntax-ns#type> <http://www.w3.org/2002/07/owl#ObjectProperty> .
_:AX2dX505cc3dcX3aX17a61a951eeX3aXX2dX7ff4 <http://www.w3.org/2002/07/owl#minCardinality> "1"^^<http://www.w3.org/2001/XMLSchema#nonNegativeInteger> .
_:AX2dX505cc3dcX3aX17a61a951eeX3aXX2dX7ff4 <http://www.w3.org/2002/07/owl#onProperty> <http://www.semanticweb.org/ontologies/2010/01/core-soa.owl#legalAspect> .
_:AX2dX505cc3dcX3aX17a61a951eeX3aXX2dX7ff4 <http://www.w3.org/1999/02/22-rdf-syntax-ns#type> <http://www.w3.org/2002/07/owl#Restriction> .
<http://www.w3id.org/ecsel-dr-AH#usesDataFormat> <http://www.w3.org/2000/01/rdf-schema#label> "uses data format"@en .
<http://www.w3id.org/ecsel-dr-AH#usesDataFormat> <http://www.w3.org/2000/01/rdf-schema#label> "This property is used to relate a service with the data format it uses."@en .
<http://www.w3id.org/ecsel-dr-AH#usesDataFormat> <http://www.w3.org/2000/01/rdf-schema#domain> <http://purl.org/dc/dcmitype/Service> .
<http://www.w3id.org/ecsel-dr-AH#usesDataFormat> <http://www.w3.org/2000/01/rdf-schema#subPropertyOf> <http://www.w3id.org/ecsel-dr-AH#usesCommTech> .
<http://www.w3id.org/ecsel-dr-AH#usesDataFormat> <http://www.w3.org/1999/02/22-rdf-syntax-ns#type> <http://www.w3.org/2002/07/owl#ObjectProperty> .
<http://www.w3id.org/ecsel-dr-AH#documents> <http://www.w3.org/2000/01/rdf-schema#label> "documents"@en .
<http://www.w3id.org/ecsel-dr-AH#documents> <http://www.w3.org/2002/07/owl#inverseOf> <http://www.w3id.org/ecsel-dr-AH#isDocumentedBy> .
<http://www.w3id.org/ecsel-dr-AH#documents> <http://www.w3.org/2000/01/rdf-schema#subPropertyOf> <http://www.w3.org/2002/07/owl#topObjectProperty> .
<http://www.w3id.org/ecsel-dr-AH#documents> <http://www.w3.org/1999/02/22-rdf-syntax-ns#type> <http://www.w3.org/2002/07/owl#ObjectProperty> .
_:AX2dX505cc3dcX3aX17a61a951eeX3aXX2dX7ffa <http://www.w3.org/1999/02/22-rdf-syntax-ns#rest> _:AX2dX505cc3dcX3aX17a61a951eeX3aXX2dX7ff9 .
_:AX2dX505cc3dcX3aX17a61a951eeX3aXX2dX7ffa <http://www.w3.org/1999/02/22-rdf-syntax-ns#first> <http://purl.org/dc/dcmitype/Software> .
