<?xml version="1.0"?>
<rdf:RDF xmlns="http://www.purl.org/i4go/variant-domain/service#"
     xml:base="http://www.purl.org/i4go/variant-domain/service"
     xmlns:rdf="http://www.w3.org/1999/02/22-rdf-syntax-ns#"
     xmlns:terms="http://purl.org/dc/terms/"
     xmlns:owl="http://www.w3.org/2002/07/owl#"
     xmlns:ns="http://creativecommons.org/ns#"
     xmlns:xml="http://www.w3.org/XML/1998/namespace"
     xmlns:xsd="http://www.w3.org/2001/XMLSchema#"
     xmlns:rdfs="http://www.w3.org/2000/01/rdf-schema#"
     xmlns:dc="http://purl.org/dc/elements/1.1/">
    <owl:Ontology rdf:about="http://www.purl.org/i4go/variant-domain/service">
        <owl:imports rdf:resource="http://www.purl.org/i4go/variant-domain/software"/>
        <rdfs:comment xml:lang="en">The &apos;Service&apos; ontology module represents the data about the functionalities provided by devices.</rdfs:comment>
        <owl:versionInfo xml:lang="en">1.0</owl:versionInfo>
        <terms:creator xml:lang="en">Javier Cuenca &lt;mailto:jcuenca@mondragon.edu&gt;
Felix Larrinaga &lt;mailto:flarrinaga@mondragon.edu&gt;</terms:creator>
        <dc:title xml:lang="en">Service ontology</dc:title>
        <terms:issued xml:lang="en">20201-05-04</terms:issued>
        <ns:license xml:lang="en">https://creativecommons.org/licenses/by-nc/4.0/</ns:license>
    </owl:Ontology>
    


    <!-- 
    ///////////////////////////////////////////////////////////////////////////////////////
    //
    // Object Properties
    //
    ///////////////////////////////////////////////////////////////////////////////////////
     -->

    


    <!-- http://www.semanticweb.org/ontologies/2010/01/core-soa.owl#hasContract -->

    <owl:ObjectProperty rdf:about="http://www.semanticweb.org/ontologies/2010/01/core-soa.owl#hasContract">
        <rdfs:subPropertyOf rdf:resource="http://www.w3.org/2002/07/owl#topObjectProperty"/>
        <owl:inverseOf rdf:resource="http://www.semanticweb.org/ontologies/2010/01/core-soa.owl#isContractFor"/>
        <rdfs:comment xml:lang="en">This property is used to relate a service with its service contract.</rdfs:comment>
        <rdfs:label xml:lang="en">has contract</rdfs:label>
    </owl:ObjectProperty>
    


    <!-- http://www.semanticweb.org/ontologies/2010/01/core-soa.owl#hasInterface -->

    <owl:ObjectProperty rdf:about="http://www.semanticweb.org/ontologies/2010/01/core-soa.owl#hasInterface">
        <rdfs:subPropertyOf rdf:resource="http://www.w3.org/2002/07/owl#topObjectProperty"/>
        <owl:inverseOf rdf:resource="http://www.semanticweb.org/ontologies/2010/01/core-soa.owl#isInterfaceOf"/>
        <rdfs:comment xml:lang="en">This property is used to relate the servicies with their interfaces</rdfs:comment>
        <rdfs:label xml:lang="en">has interface</rdfs:label>
    </owl:ObjectProperty>
    


    <!-- http://www.semanticweb.org/ontologies/2010/01/core-soa.owl#isContractFor -->

    <owl:ObjectProperty rdf:about="http://www.semanticweb.org/ontologies/2010/01/core-soa.owl#isContractFor">
        <rdfs:subPropertyOf rdf:resource="http://www.w3.org/2002/07/owl#topObjectProperty"/>
        <rdfs:label xml:lang="en">is contract for</rdfs:label>
    </owl:ObjectProperty>
    


    <!-- http://www.semanticweb.org/ontologies/2010/01/core-soa.owl#isInterfaceOf -->

    <owl:ObjectProperty rdf:about="http://www.semanticweb.org/ontologies/2010/01/core-soa.owl#isInterfaceOf">
        <rdfs:subPropertyOf rdf:resource="http://www.w3.org/2002/07/owl#topObjectProperty"/>
        <rdfs:label xml:lang="en">is interface of</rdfs:label>
    </owl:ObjectProperty>
    


    <!-- http://www.semanticweb.org/ontologies/2010/01/core-soa.owl#isSpecifiedBy -->

    <owl:ObjectProperty rdf:about="http://www.semanticweb.org/ontologies/2010/01/core-soa.owl#isSpecifiedBy">
        <rdfs:subPropertyOf rdf:resource="http://www.w3.org/2002/07/owl#topObjectProperty"/>
        <rdfs:label xml:lang="en">is specified by</rdfs:label>
    </owl:ObjectProperty>
    


    <!-- http://www.semanticweb.org/ontologies/2010/01/core-soa.owl#specifies -->

    <owl:ObjectProperty rdf:about="http://www.semanticweb.org/ontologies/2010/01/core-soa.owl#specifies">
        <rdfs:subPropertyOf rdf:resource="http://www.w3.org/2002/07/owl#topObjectProperty"/>
        <rdfs:comment xml:lang="en">This property relates a service contract with the effect it specifies.</rdfs:comment>
        <rdfs:label xml:lang="en">specifies</rdfs:label>
    </owl:ObjectProperty>
    


    <!-- http://www.w3.org/2002/07/owl#topObjectProperty -->

    <rdf:Description rdf:about="http://www.w3.org/2002/07/owl#topObjectProperty">
        <rdfs:domain rdf:resource="http://purl.org/dc/dcmitype/Service"/>
        <rdfs:range rdf:resource="http://www.w3id.org/ecsel-dr-AH#Method"/>
    </rdf:Description>
    


    <!-- http://www.w3id.org/ecsel-dr-AH#documents -->

    <owl:ObjectProperty rdf:about="http://www.w3id.org/ecsel-dr-AH#documents">
        <rdfs:subPropertyOf rdf:resource="http://www.w3.org/2002/07/owl#topObjectProperty"/>
        <owl:inverseOf rdf:resource="http://www.w3id.org/ecsel-dr-AH#isDocumentedBy"/>
        <rdfs:label xml:lang="en">documents</rdfs:label>
    </owl:ObjectProperty>
    


    <!-- http://www.w3id.org/ecsel-dr-AH#hasInformationModel -->

    <owl:ObjectProperty rdf:about="http://www.w3id.org/ecsel-dr-AH#hasInformationModel">
        <rdfs:subPropertyOf rdf:resource="http://www.w3.org/2002/07/owl#topObjectProperty"/>
        <owl:inverseOf rdf:resource="http://www.w3id.org/ecsel-dr-AH#isInformationModelOf"/>
        <rdfs:domain rdf:resource="http://purl.org/dc/dcmitype/Service"/>
        <rdfs:range rdf:resource="http://www.w3id.org/ecsel-dr-AH#InformationModel"/>
        <rdfs:comment xml:lang="en">This property is used to relate services with their information model.</rdfs:comment>
        <rdfs:label xml:lang="en">has information model</rdfs:label>
    </owl:ObjectProperty>
    


    <!-- http://www.w3id.org/ecsel-dr-AH#hasMethod -->

    <owl:ObjectProperty rdf:about="http://www.w3id.org/ecsel-dr-AH#hasMethod">
        <rdfs:subPropertyOf rdf:resource="http://www.w3.org/2002/07/owl#topObjectProperty"/>
        <owl:inverseOf rdf:resource="http://www.w3id.org/ecsel-dr-AH#isMethodOf"/>
        <rdfs:comment xml:lang="en">This property is used to relate servicies with the methods they provide.</rdfs:comment>
        <rdfs:label xml:lang="en">has method</rdfs:label>
    </owl:ObjectProperty>
    


    <!-- http://www.w3id.org/ecsel-dr-AH#isDocumentedBy -->

    <owl:ObjectProperty rdf:about="http://www.w3id.org/ecsel-dr-AH#isDocumentedBy">
        <rdfs:subPropertyOf rdf:resource="http://www.w3.org/2002/07/owl#topObjectProperty"/>
        <rdfs:domain>
            <owl:Class>
                <owl:unionOf rdf:parseType="Collection">
                    <rdf:Description rdf:about="http://purl.org/dc/dcmitype/Service"/>
                    <rdf:Description rdf:about="http://purl.org/dc/dcmitype/Software"/>
                    <rdf:Description rdf:about="http://www.w3id.org/ecsel-dr-AH#System-of-Systems"/>
                </owl:unionOf>
            </owl:Class>
        </rdfs:domain>
        <rdfs:range rdf:resource="http://www.purl.org/i4go/common-domain/system/SystemDocumentation"/>
        <rdfs:range rdf:resource="http://www.purl.org/i4go/variant-domain/service/ServiceDocumentation"/>
        <rdfs:comment xml:lang="en">This property is used to relate systems and services with their documentation</rdfs:comment>
        <rdfs:label xml:lang="en">is documented by</rdfs:label>
    </owl:ObjectProperty>
    


    <!-- http://www.w3id.org/ecsel-dr-AH#isInformationModelOf -->

    <owl:ObjectProperty rdf:about="http://www.w3id.org/ecsel-dr-AH#isInformationModelOf">
        <rdfs:subPropertyOf rdf:resource="http://www.w3.org/2002/07/owl#topObjectProperty"/>
        <rdfs:label xml:lang="en">is information model of</rdfs:label>
    </owl:ObjectProperty>
    


    <!-- http://www.w3id.org/ecsel-dr-AH#isMethodOf -->

    <owl:ObjectProperty rdf:about="http://www.w3id.org/ecsel-dr-AH#isMethodOf">
        <rdfs:subPropertyOf rdf:resource="http://www.w3.org/2002/07/owl#topObjectProperty"/>
        <rdfs:label xml:lang="en">is method of</rdfs:label>
    </owl:ObjectProperty>
    


    <!-- http://www.w3id.org/ecsel-dr-AH#isServiceProducerOf -->

    <owl:ObjectProperty rdf:about="http://www.w3id.org/ecsel-dr-AH#isServiceProducerOf">
        <rdfs:subPropertyOf rdf:resource="http://www.w3.org/2002/07/owl#topObjectProperty"/>
        <owl:inverseOf rdf:resource="http://www.w3id.org/ecsel-dr-AH#producedBy"/>
        <rdfs:label xml:lang="en">is service producer of</rdfs:label>
    </owl:ObjectProperty>
    


    <!-- http://www.w3id.org/ecsel-dr-AH#producedBy -->

    <owl:ObjectProperty rdf:about="http://www.w3id.org/ecsel-dr-AH#producedBy">
        <rdfs:subPropertyOf rdf:resource="http://www.w3.org/2002/07/owl#topObjectProperty"/>
        <owl:inverseOf rdf:resource="http://www.w3id.org/ecsel-dr-AH#produces"/>
        <rdfs:domain rdf:resource="http://purl.org/dc/dcmitype/Service"/>
        <rdfs:range rdf:resource="http://purl.org/dc/dcmitype/Software"/>
        <rdfs:comment xml:lang="en">This property relates the servicies with the software systems that provide them.</rdfs:comment>
        <rdfs:label xml:lang="en">produced by</rdfs:label>
    </owl:ObjectProperty>
    


    <!-- http://www.w3id.org/ecsel-dr-AH#produces -->

    <owl:ObjectProperty rdf:about="http://www.w3id.org/ecsel-dr-AH#produces">
        <rdfs:subPropertyOf rdf:resource="http://www.w3.org/2002/07/owl#topObjectProperty"/>
        <rdfs:comment xml:lang="en">Relation expressing that a software system produces a service. 
Equivalent names for this relation include
- offers
- provides 
- isServiceProducerOf 
Since Arrowhead uses the pair produce / consume and corresponding service producer / service consumer adressing the relations and the software systems, this ontology uses these names for the relations too. 
If it is needed, object properties with other names can be added and stated to be equivalent to these ones.</rdfs:comment>
        <rdfs:label xml:lang="en">produces</rdfs:label>
    </owl:ObjectProperty>
    


    <!-- http://www.w3id.org/ecsel-dr-AH#usesCommTech -->

    <owl:ObjectProperty rdf:about="http://www.w3id.org/ecsel-dr-AH#usesCommTech">
        <rdfs:subPropertyOf rdf:resource="http://www.w3.org/2002/07/owl#topObjectProperty"/>
        <rdfs:domain rdf:resource="http://purl.org/dc/dcmitype/Service"/>
        <rdfs:range rdf:resource="http://www.purl.org/i4go/variant-domain/service/CommunicationTechnology"/>
        <rdfs:comment xml:lang="en">This property is used to relate a service with the communication technology it uses.</rdfs:comment>
        <rdfs:label xml:lang="en">uses communication technology</rdfs:label>
    </owl:ObjectProperty>
    


    <!-- http://www.w3id.org/ecsel-dr-AH#usesDataFormat -->

    <owl:ObjectProperty rdf:about="http://www.w3id.org/ecsel-dr-AH#usesDataFormat">
        <rdfs:subPropertyOf rdf:resource="http://www.w3id.org/ecsel-dr-AH#usesCommTech"/>
        <rdfs:domain rdf:resource="http://purl.org/dc/dcmitype/Service"/>
        <rdfs:label xml:lang="en">This property is used to relate a service with the data format it uses.</rdfs:label>
        <rdfs:label xml:lang="en">uses data format</rdfs:label>
    </owl:ObjectProperty>
    


    <!-- http://www.w3id.org/ecsel-dr-AH#usesSecurityMechanism -->

    <owl:ObjectProperty rdf:about="http://www.w3id.org/ecsel-dr-AH#usesSecurityMechanism">
        <rdfs:subPropertyOf rdf:resource="http://www.w3id.org/ecsel-dr-AH#usesCommTech"/>
        <rdfs:domain rdf:resource="http://purl.org/dc/dcmitype/Service"/>
        <rdfs:range rdf:resource="http://www.purl.org/i4go/variant-domain/service/CommunicationSecurityMechanism"/>
        <rdfs:comment xml:lang="en">This property is used to relate a service with the security mechanism it uses.</rdfs:comment>
        <rdfs:label xml:lang="en">uses security mechanism</rdfs:label>
    </owl:ObjectProperty>
    


    <!-- http://www.w3id.org/ecsel-dr-AH#usesTransferProtocol -->

    <owl:ObjectProperty rdf:about="http://www.w3id.org/ecsel-dr-AH#usesTransferProtocol">
        <rdfs:subPropertyOf rdf:resource="http://www.w3id.org/ecsel-dr-AH#usesCommTech"/>
        <rdfs:comment xml:lang="en">This property is used to relate a service with the data transfer protocol it uses.</rdfs:comment>
        <rdfs:label xml:lang="en">uses transfer protocol</rdfs:label>
    </owl:ObjectProperty>
    


    <!-- 
    ///////////////////////////////////////////////////////////////////////////////////////
    //
    // Data properties
    //
    ///////////////////////////////////////////////////////////////////////////////////////
     -->

    


    <!-- http://www.semanticweb.org/ontologies/2010/01/core-soa.owl#constraints -->

    <owl:DatatypeProperty rdf:about="http://www.semanticweb.org/ontologies/2010/01/core-soa.owl#constraints">
        <rdfs:subPropertyOf rdf:resource="http://www.w3.org/2002/07/owl#topDataProperty"/>
        <rdfs:domain rdf:resource="http://www.semanticweb.org/ontologies/2010/01/core-soa.owl#ServiceInterface"/>
        <rdfs:label xml:lang="en">constraints</rdfs:label>
    </owl:DatatypeProperty>
    


    <!-- http://www.semanticweb.org/ontologies/2010/01/core-soa.owl#interactionAspect -->

    <owl:DatatypeProperty rdf:about="http://www.semanticweb.org/ontologies/2010/01/core-soa.owl#interactionAspect">
        <rdfs:subPropertyOf rdf:resource="http://www.w3.org/2002/07/owl#topDataProperty"/>
        <rdfs:domain rdf:resource="http://www.semanticweb.org/ontologies/2010/01/core-soa.owl#ServiceContract"/>
        <rdfs:label xml:lang="en">interfaction aspect</rdfs:label>
    </owl:DatatypeProperty>
    


    <!-- http://www.semanticweb.org/ontologies/2010/01/core-soa.owl#legalAspect -->

    <owl:DatatypeProperty rdf:about="http://www.semanticweb.org/ontologies/2010/01/core-soa.owl#legalAspect">
        <rdfs:subPropertyOf rdf:resource="http://www.w3.org/2002/07/owl#topDataProperty"/>
        <rdfs:domain rdf:resource="http://www.semanticweb.org/ontologies/2010/01/core-soa.owl#ServiceContract"/>
        <rdfs:label xml:lang="en">legal aspect</rdfs:label>
    </owl:DatatypeProperty>
    


    <!-- 
    ///////////////////////////////////////////////////////////////////////////////////////
    //
    // Classes
    //
    ///////////////////////////////////////////////////////////////////////////////////////
     -->

    


    <!-- http://purl.org/dc/dcmitype/Service -->

    <owl:Class rdf:about="http://purl.org/dc/dcmitype/Service">
        <rdfs:subClassOf>
            <owl:Restriction>
                <owl:onProperty rdf:resource="http://www.semanticweb.org/ontologies/2010/01/core-soa.owl#hasInterface"/>
                <owl:minCardinality rdf:datatype="http://www.w3.org/2001/XMLSchema#nonNegativeInteger">1</owl:minCardinality>
            </owl:Restriction>
        </rdfs:subClassOf>
        <rdfs:comment xml:lang="en">Distinct part of the functionality that is provided by an entity through interfaces</rdfs:comment>
        <rdfs:label xml:lang="en">Service</rdfs:label>
    </owl:Class>
    


    <!-- http://purl.org/ontology/is/core#InfoService -->

    <owl:Class rdf:about="http://purl.org/ontology/is/core#InfoService">
        <rdfs:subClassOf rdf:resource="http://purl.org/dc/dcmitype/Service"/>
        <rdfs:comment xml:lang="en">Service offered by a system that provides information</rdfs:comment>
        <rdfs:label xml:lang="en">Info service</rdfs:label>
    </owl:Class>
    


    <!-- http://www.purl.org/i4go/variant-domain/service/CommunicationSecurityMechanism -->

    <owl:Class rdf:about="http://www.purl.org/i4go/variant-domain/service/CommunicationSecurityMechanism">
        <rdfs:subClassOf rdf:resource="http://www.purl.org/i4go/variant-domain/service/CommunicationTechnology"/>
        <rdfs:comment xml:lang="en">Corresponds to a part of OSI layer 5</rdfs:comment>
        <rdfs:label xml:lang="en">Communication technology mecanism</rdfs:label>
    </owl:Class>
    


    <!-- http://www.purl.org/i4go/variant-domain/service/CommunicationTechnology -->

    <owl:Class rdf:about="http://www.purl.org/i4go/variant-domain/service/CommunicationTechnology">
        <rdfs:comment xml:lang="en">The communication technology used by a service.</rdfs:comment>
        <rdfs:label xml:lang="en">Communication technology</rdfs:label>
    </owl:Class>
    


    <!-- http://www.purl.org/i4go/variant-domain/service/DataFormat -->

    <owl:Class rdf:about="http://www.purl.org/i4go/variant-domain/service/DataFormat">
        <rdfs:comment xml:lang="en">This class is used to represent any data format.</rdfs:comment>
        <rdfs:label xml:lang="en">Data format</rdfs:label>
    </owl:Class>
    


    <!-- http://www.purl.org/i4go/variant-domain/service/DataLinkAndMediaAccessTechnology -->

    <owl:Class rdf:about="http://www.purl.org/i4go/variant-domain/service/DataLinkAndMediaAccessTechnology">
        <rdfs:subClassOf rdf:resource="http://www.purl.org/i4go/variant-domain/service/CommunicationTechnology"/>
        <rdfs:comment xml:lang="en">Corresponds to OSI layer 1 and 2 technologies, like Ethernet, WLAN (802.11), WPAN (802.15.4), EtherCAT, ProfiNet, ...</rdfs:comment>
        <rdfs:label xml:lang="en">Data link and media access technology</rdfs:label>
    </owl:Class>
    


    <!-- http://www.purl.org/i4go/variant-domain/service/End-to-EndCommunicationTechnology -->

    <owl:Class rdf:about="http://www.purl.org/i4go/variant-domain/service/End-to-EndCommunicationTechnology">
        <rdfs:subClassOf rdf:resource="http://www.purl.org/i4go/variant-domain/service/CommunicationTechnology"/>
        <rdfs:comment xml:lang="en">The end-to-end principle is a network design method in which application-specific features are kept at communication end points.</rdfs:comment>
        <rdfs:label xml:lang="en">End-to-end communication technology</rdfs:label>
    </owl:Class>
    


    <!-- http://www.purl.org/i4go/variant-domain/service/Point-to-PointCommunicationTechnology -->

    <owl:Class rdf:about="http://www.purl.org/i4go/variant-domain/service/Point-to-PointCommunicationTechnology">
        <rdfs:subClassOf rdf:resource="http://www.purl.org/i4go/variant-domain/service/CommunicationTechnology"/>
        <rdfs:comment xml:lang="en">In telecommunications, a point-to-point connection refers to a communications connection between two communication endpoints or nodes. An example is a telephone call, in which one telephone is connected with one other, and what is said by one caller can only be heard by the other.</rdfs:comment>
        <rdfs:label xml:lang="en">Point-to-point communication technology</rdfs:label>
    </owl:Class>
    


    <!-- http://www.purl.org/i4go/variant-domain/service/ServiceDocumentation -->

    <owl:Class rdf:about="http://www.purl.org/i4go/variant-domain/service/ServiceDocumentation">
        <rdfs:comment xml:lang="en">Collection of documents that contain the information about a service.</rdfs:comment>
        <rdfs:label xml:lang="en">Service documentation</rdfs:label>
    </owl:Class>
    


    <!-- http://www.purl.org/i4go/variant-domain/service/TransferProtocol -->

    <owl:Class rdf:about="http://www.purl.org/i4go/variant-domain/service/TransferProtocol">
        <rdfs:subClassOf rdf:resource="http://www.purl.org/i4go/variant-domain/service/CommunicationTechnology"/>
        <rdfs:comment xml:lang="en">This class is used to reptresent a data transfer protocol.</rdfs:comment>
        <rdfs:label xml:lang="en">Transfer protocol</rdfs:label>
    </owl:Class>
    


    <!-- http://www.semanticweb.org/ontologies/2010/01/core-soa.owl#Effect -->

    <owl:Class rdf:about="http://www.semanticweb.org/ontologies/2010/01/core-soa.owl#Effect">
        <rdfs:comment xml:lang="en">The effect of a service contract.</rdfs:comment>
        <rdfs:label xml:lang="en">Effect</rdfs:label>
    </owl:Class>
    


    <!-- http://www.semanticweb.org/ontologies/2010/01/core-soa.owl#ServiceContract -->

    <owl:Class rdf:about="http://www.semanticweb.org/ontologies/2010/01/core-soa.owl#ServiceContract">
        <rdfs:subClassOf>
            <owl:Restriction>
                <owl:onProperty rdf:resource="http://www.semanticweb.org/ontologies/2010/01/core-soa.owl#isContractFor"/>
                <owl:minCardinality rdf:datatype="http://www.w3.org/2001/XMLSchema#nonNegativeInteger">1</owl:minCardinality>
            </owl:Restriction>
        </rdfs:subClassOf>
        <rdfs:subClassOf>
            <owl:Restriction>
                <owl:onProperty rdf:resource="http://www.semanticweb.org/ontologies/2010/01/core-soa.owl#specifies"/>
                <owl:minCardinality rdf:datatype="http://www.w3.org/2001/XMLSchema#nonNegativeInteger">1</owl:minCardinality>
            </owl:Restriction>
        </rdfs:subClassOf>
        <rdfs:subClassOf>
            <owl:Restriction>
                <owl:onProperty rdf:resource="http://www.semanticweb.org/ontologies/2010/01/core-soa.owl#interactionAspect"/>
                <owl:minCardinality rdf:datatype="http://www.w3.org/2001/XMLSchema#nonNegativeInteger">1</owl:minCardinality>
            </owl:Restriction>
        </rdfs:subClassOf>
        <rdfs:subClassOf>
            <owl:Restriction>
                <owl:onProperty rdf:resource="http://www.semanticweb.org/ontologies/2010/01/core-soa.owl#legalAspect"/>
                <owl:minCardinality rdf:datatype="http://www.w3.org/2001/XMLSchema#nonNegativeInteger">1</owl:minCardinality>
            </owl:Restriction>
        </rdfs:subClassOf>
        <rdfs:subClassOf>
            <owl:Restriction>
                <owl:onProperty rdf:resource="http://www.semanticweb.org/ontologies/2010/01/core-soa.owl#interactionAspect"/>
                <owl:maxCardinality rdf:datatype="http://www.w3.org/2001/XMLSchema#nonNegativeInteger">1</owl:maxCardinality>
            </owl:Restriction>
        </rdfs:subClassOf>
        <rdfs:subClassOf>
            <owl:Restriction>
                <owl:onProperty rdf:resource="http://www.semanticweb.org/ontologies/2010/01/core-soa.owl#legalAspect"/>
                <owl:maxCardinality rdf:datatype="http://www.w3.org/2001/XMLSchema#nonNegativeInteger">1</owl:maxCardinality>
            </owl:Restriction>
        </rdfs:subClassOf>
        <rdfs:comment xml:lang="en">Is a document that sets out the provision and delivery of software services to customers through the internet.</rdfs:comment>
        <rdfs:label xml:lang="en">Service contract</rdfs:label>
    </owl:Class>
    


    <!-- http://www.semanticweb.org/ontologies/2010/01/core-soa.owl#ServiceInterface -->

    <owl:Class rdf:about="http://www.semanticweb.org/ontologies/2010/01/core-soa.owl#ServiceInterface">
        <rdfs:subClassOf>
            <owl:Restriction>
                <owl:onProperty rdf:resource="http://www.semanticweb.org/ontologies/2010/01/core-soa.owl#constraints"/>
                <owl:minCardinality rdf:datatype="http://www.w3.org/2001/XMLSchema#nonNegativeInteger">1</owl:minCardinality>
            </owl:Restriction>
        </rdfs:subClassOf>
        <rdfs:subClassOf>
            <owl:Restriction>
                <owl:onProperty rdf:resource="http://www.semanticweb.org/ontologies/2010/01/core-soa.owl#constraints"/>
                <owl:maxCardinality rdf:datatype="http://www.w3.org/2001/XMLSchema#nonNegativeInteger">1</owl:maxCardinality>
            </owl:Restriction>
        </rdfs:subClassOf>
        <rdfs:comment xml:lang="en">A service interface is a published interface used to invoke a service. An interface can be implemented using any number of technologies, including WSDL, XML-RPC, COM+, CORBA (IDL), Java RMI, and others. A service interface can be described using multiple methods.</rdfs:comment>
        <rdfs:label xml:lang="en">Service interface</rdfs:label>
    </owl:Class>
    


    <!-- http://www.w3id.org/ecsel-dr-AH#InformationModel -->

    <owl:Class rdf:about="http://www.w3id.org/ecsel-dr-AH#InformationModel">
        <rdfs:comment xml:lang="en">An information model in software engineering is a representation of concepts and the relationships, constraints, rules, and operations to specify data semantics for a chosen domain of discourse.</rdfs:comment>
        <rdfs:label xml:lang="en">Information model</rdfs:label>
    </owl:Class>
    


    <!-- http://www.w3id.org/ecsel-dr-AH#Method -->

    <owl:Class rdf:about="http://www.w3id.org/ecsel-dr-AH#Method">
        <rdfs:comment xml:lang="en">Method of a service: method that is provided by a service within a SoA.</rdfs:comment>
        <rdfs:label xml:lang="en">Method</rdfs:label>
    </owl:Class>
    


    <!-- http://www.w3id.org/ecsel-dr-PMV#OtherServices -->

    <owl:Class rdf:about="http://www.w3id.org/ecsel-dr-PMV#OtherServices">
        <rdfs:subClassOf rdf:resource="http://purl.org/dc/dcmitype/Service"/>
        <rdfs:comment xml:lang="en">Collection of other services used as input to a production process or which are created during a production process.</rdfs:comment>
        <rdfs:label xml:lang="en">Other services</rdfs:label>
    </owl:Class>
</rdf:RDF>



<!-- Generated by the OWL API (version 4.2.6.20160910-2108) https://github.com/owlcs/owlapi -->

