@prefix :        <http://www.purl.org/i40go/domain-task/customer#> .
@prefix owl:     <http://www.w3.org/2002/07/owl#> .
@prefix rdf:     <http://www.w3.org/1999/02/22-rdf-syntax-ns#> .
@prefix terms:   <http://purl.org/dc/terms/> .
@prefix ns:      <http://creativecommons.org/ns#> .
@prefix xsd:     <http://www.w3.org/2001/XMLSchema#> .
@prefix rdfs:    <http://www.w3.org/2000/01/rdf-schema#> .
@prefix dc:      <http://purl.org/dc/elements/1.1/> .

<http://www.w3id.org/ecsel-dr-OM#CustomerPlant>
      a       owl:Class ;
      rdfs:label "Customer plant"@en .

<http://www.w3id.org/ecsel-dr-OM#requestsOrderChangeRequest>
      a       owl:ObjectProperty ;
      rdfs:comment "This property relates a customer with an order change request."@en ;
      rdfs:domain <http://www.w3id.org/ecsel-dr-OM#Customer> ;
      rdfs:label "requests order change request"@en ;
      rdfs:subPropertyOf owl:topObjectProperty .

<http://www.purl.org/i40go/domain-task/customer/DemandSnapshot>
      a       owl:Class ;
      rdfs:comment "The “Demand” entity stores redundant demand at every product level."@en ;
      rdfs:label "Demand snapshot"@en .

<http://www.w3id.org/ecsel-dr-PROD#customerPartNumber>
      a       owl:DatatypeProperty ;
      rdfs:comment "Product identifier used by the customer to identify one IFX product"@en ;
      rdfs:label "customer part number"@en ;
      rdfs:subPropertyOf owl:topDataProperty .

<http://www.w3id.org/ecsel-dr-OM#ownsCustomerPlant>
      a       owl:ObjectProperty ;
      rdfs:label "owns customer plant"@en ;
      rdfs:subPropertyOf owl:topObjectProperty .

<http://www.w3id.org/ecsel-dr-OM#Customer>
      a       owl:Class ;
      rdfs:comment "The purchaser/user of a product or service supplied by a service provider or utility."@en ;
      rdfs:label "Customer"@en .

owl:topDataProperty
      rdfs:range xsd:string .

ns:license
      a       owl:AnnotationProperty .

<http://www.w3id.org/ecsel-dr-OM#CustomerData>
      a       owl:Class ;
      rdfs:comment "This class is used to represent any information about a customer"@en ;
      rdfs:label "Customer data"@en .

<http://www.w3id.org/ecsel-dr-SO#hasCustomerWishTime>
      a       owl:DatatypeProperty ;
      rdfs:comment "Customer wish time of the demand entry"@en ;
      rdfs:label "has customer wish time"@en ;
      rdfs:subPropertyOf owl:topDataProperty .

terms:issued
      a       owl:AnnotationProperty .

<http://www.w3id.org/ecsel-dr-PROD#customer>
      a       owl:ObjectProperty ;
      rdfs:comment "This property is used to indicate the customer of an organization"@en ;
      rdfs:label "customer"@en ;
      rdfs:range <http://www.w3id.org/ecsel-dr-PROD#Organization> ;
      rdfs:subPropertyOf owl:topObjectProperty .

terms:creator
      a       owl:AnnotationProperty .

<http://www.purl.org/i40go/domain-task/customer>
      a       owl:Ontology ;
      rdfs:comment "The 'Customer' ontology module represents data about the customers of the organization products."@en ;
      ns:license "https://creativecommons.org/licenses/by-nc/4.0/"@en ;
      dc:title "Customer ontology"@en ;
      terms:creator """Javier Cuenca <mailto:jcuenca@mondragon.edu>
Felix Larrinaga <mailto:flarrinaga@mondragon.edu>"""@en ;
      terms:issued "2021-25-05"@en ;
      owl:imports <http://www.purl.org/i40go/common-domain/organization> ;
      owl:versionInfo "1.0"@en .

<http://www.w3id.org/ecsel-dr-OM#OrderChangeRequest>
      a       owl:Class ;
      rdfs:comment "Change Order Request (COR means a Contractor generated document which describes a change in the scope of Work, including a detailed description, Drawings and Specifications, and a request for changes to costs or time, as necessary, to inform Owner of the nature of the requested change to the Contract."@en ;
      rdfs:label "Order change request"@en .
