<http://www.w3id.org/ecsel-dr-SO#hasSplitLotChips> <http://www.w3.org/2000/01/rdf-schema#label> "has split lot chips"@en .
<http://www.w3id.org/ecsel-dr-SO#hasSplitLotChips> <http://www.w3.org/2000/01/rdf-schema#comment> "Split into lots with # chips, added due to data import"@en .
<http://www.w3id.org/ecsel-dr-SO#hasSplitLotChips> <http://www.w3.org/2000/01/rdf-schema#range> <http://www.w3.org/2001/XMLSchema#integer> .
<http://www.w3id.org/ecsel-dr-SO#hasSplitLotChips> <http://www.w3.org/2000/01/rdf-schema#domain> <http://www.w3id.org/ecsel-dr-SO#Operation> .
<http://www.w3id.org/ecsel-dr-SO#hasSplitLotChips> <http://www.w3.org/2000/01/rdf-schema#subPropertyOf> <http://www.w3.org/2002/07/owl#topDataProperty> .
<http://www.w3id.org/ecsel-dr-SO#hasSplitLotChips> <http://www.w3.org/1999/02/22-rdf-syntax-ns#type> <http://www.w3.org/2002/07/owl#DatatypeProperty> .
<http://www.w3id.org/ecsel-dr-SO#hasCurrentWIP> <http://www.w3.org/2000/01/rdf-schema#label> "has current WIP"@en .
<http://www.w3id.org/ecsel-dr-SO#hasCurrentWIP> <http://www.w3.org/2000/01/rdf-schema#comment> "This property is used to relate operations with their current WIP."@en .
<http://www.w3id.org/ecsel-dr-SO#hasCurrentWIP> <http://www.w3.org/2000/01/rdf-schema#range> <http://www.w3id.org/ecsel-dr-SO#CurrentWIP> .
<http://www.w3id.org/ecsel-dr-SO#hasCurrentWIP> <http://www.w3.org/2000/01/rdf-schema#domain> _:A6b5d418bX3aX17a61612d50X3aXX2dX7ffc .
<http://www.w3id.org/ecsel-dr-SO#hasCurrentWIP> <http://www.w3.org/2000/01/rdf-schema#subPropertyOf> <http://www.w3.org/2002/07/owl#topObjectProperty> .
<http://www.w3id.org/ecsel-dr-SO#hasCurrentWIP> <http://www.w3.org/1999/02/22-rdf-syntax-ns#type> <http://www.w3.org/2002/07/owl#ObjectProperty> .
<http://www.purl.org/i4go/variant-domain/operation/TimeConstraints> <http://www.w3.org/2000/01/rdf-schema#label> "Time constraints"@en .
<http://www.purl.org/i4go/variant-domain/operation/TimeConstraints> <http://www.w3.org/2000/01/rdf-schema#comment> "As single operations can set the lot to a time-critical state, time constraints can ensure that the operation setting it to an uncritical state is not delayed. Also the other case where certain time has to be spent between two operations can be covered with this master entity. (workflow deswcriptive master entities)."@en .
<http://www.purl.org/i4go/variant-domain/operation/TimeConstraints> <http://www.w3.org/1999/02/22-rdf-syntax-ns#type> <http://www.w3.org/2002/07/owl#Class> .
<http://www.purl.org/i4go/variant-domain/operation/OperatingProperty> <http://www.w3.org/2000/01/rdf-schema#label> "Operating property"@en .
<http://www.purl.org/i4go/variant-domain/operation/OperatingProperty> <http://www.w3.org/2000/01/rdf-schema#comment> "This class is used to represent operation and configuration aspects of devices."@en .
<http://www.purl.org/i4go/variant-domain/operation/OperatingProperty> <http://www.w3.org/2000/01/rdf-schema#subClassOf> <http://www.w3.org/ns/ssn/Property> .
<http://www.purl.org/i4go/variant-domain/operation/OperatingProperty> <http://www.w3.org/1999/02/22-rdf-syntax-ns#type> <http://www.w3.org/2002/07/owl#Class> .
<http://www.w3id.org/ecsel-dr-SO#isOperationOf> <http://www.w3.org/2000/01/rdf-schema#label> "is operation of"@en .
<http://www.w3id.org/ecsel-dr-SO#isOperationOf> <http://www.w3.org/2000/01/rdf-schema#subPropertyOf> <http://www.w3.org/2002/07/owl#topObjectProperty> .
<http://www.w3id.org/ecsel-dr-SO#isOperationOf> <http://www.w3.org/1999/02/22-rdf-syntax-ns#type> <http://www.w3.org/2002/07/owl#ObjectProperty> .
<http://www.w3id.org/ecsel-dr-PWR#Enhancement> <http://www.w3.org/2000/01/rdf-schema#label> "Enhancement mode"@en .
<http://www.w3id.org/ecsel-dr-PWR#Enhancement> <http://www.w3.org/2000/01/rdf-schema#comment> "A transistor that is normally open (off), but is triggered to close (on)."@en .
<http://www.w3id.org/ecsel-dr-PWR#Enhancement> <http://www.w3.org/2000/01/rdf-schema#subClassOf> <http://www.purl.org/i4go/variant-domain/operation/OperationMode> .
<http://www.w3id.org/ecsel-dr-PWR#Enhancement> <http://www.w3.org/1999/02/22-rdf-syntax-ns#type> <http://www.w3.org/2002/07/owl#Class> .
_:A6b5d418bX3aX17a61612d50X3aXX2dX7ffb <http://www.w3.org/1999/02/22-rdf-syntax-ns#rest> _:A6b5d418bX3aX17a61612d50X3aXX2dX7ffa .
_:A6b5d418bX3aX17a61612d50X3aXX2dX7ffb <http://www.w3.org/1999/02/22-rdf-syntax-ns#first> <http://www.purl.org/i4go/variant-domain/operation/EventCalendar> .
<http://www.purl.org/i4go/variant-domain/operation/DryEtching> <http://www.w3.org/2000/01/rdf-schema#label> "Dry etching"@en .
<http://www.purl.org/i4go/variant-domain/operation/DryEtching> <http://www.w3.org/2000/01/rdf-schema#comment> "Dry etching is a process whereby etching is accomplished by a reactive gas as opposed to a liquid. Dry etching techniques include plasma etch, reactive ion etch, magnetically enhanced reactive ion etch, inductively coupled plasma, electron spin resonance, etc."@en .
<http://www.purl.org/i4go/variant-domain/operation/DryEtching> <http://www.w3.org/2000/01/rdf-schema#subClassOf> <http://www.w3id.org/ecsel-dr-SO#Workshop> .
<http://www.purl.org/i4go/variant-domain/operation/DryEtching> <http://www.w3.org/1999/02/22-rdf-syntax-ns#type> <http://www.w3.org/2002/07/owl#Class> .
<http://www.w3id.org/ecsel-dr-SO#hasSupplyChainID> <http://www.w3.org/2000/01/rdf-schema#label> "has supply chain id"@en .
<http://www.w3id.org/ecsel-dr-SO#hasSupplyChainID> <http://www.w3.org/2000/01/rdf-schema#comment> "Assignment of technology to supply chain."@en .
<http://www.w3id.org/ecsel-dr-SO#hasSupplyChainID> <http://www.w3.org/2000/01/rdf-schema#range> <http://www.w3.org/2001/XMLSchema#string> .
<http://www.w3id.org/ecsel-dr-SO#hasSupplyChainID> <http://www.w3.org/2000/01/rdf-schema#domain> <http://www.w3id.org/ecsel-dr-SO#Technology> .
<http://www.w3id.org/ecsel-dr-SO#hasSupplyChainID> <http://www.w3.org/2000/01/rdf-schema#subPropertyOf> <http://www.w3.org/2002/07/owl#topDataProperty> .
<http://www.w3id.org/ecsel-dr-SO#hasSupplyChainID> <http://www.w3.org/1999/02/22-rdf-syntax-ns#type> <http://www.w3.org/2002/07/owl#DatatypeProperty> .
<http://www.w3id.org/ecsel-dr-SO#hasOperation> <http://www.w3.org/2000/01/rdf-schema#label> "has operation"@en .
<http://www.w3id.org/ecsel-dr-SO#hasOperation> <http://www.w3.org/2000/01/rdf-schema#comment> "This property is used to relate different entities (such as equipment) the the operations they perform."@en .
<http://www.w3id.org/ecsel-dr-SO#hasOperation> <http://www.w3.org/2000/01/rdf-schema#range> <http://www.w3id.org/ecsel-dr-SO#Operation> .
<http://www.w3id.org/ecsel-dr-SO#hasOperation> <http://www.w3.org/2000/01/rdf-schema#domain> _:A6b5d418bX3aX17a61612d50X3aXX2dX7ff3 .
<http://www.w3id.org/ecsel-dr-SO#hasOperation> <http://www.w3.org/2002/07/owl#inverseOf> <http://www.w3id.org/ecsel-dr-SO#isOperationOf> .
<http://www.w3id.org/ecsel-dr-SO#hasOperation> <http://www.w3.org/2000/01/rdf-schema#subPropertyOf> <http://www.w3.org/2002/07/owl#topObjectProperty> .
<http://www.w3id.org/ecsel-dr-SO#hasOperation> <http://www.w3.org/1999/02/22-rdf-syntax-ns#type> <http://www.w3.org/2002/07/owl#ObjectProperty> .
<http://www.purl.org/i4go/variant-domain/operation/SimulationRoute> <http://www.w3.org/2000/01/rdf-schema#label> "Simulation route"@en .
<http://www.purl.org/i4go/variant-domain/operation/SimulationRoute> <http://www.w3.org/2000/01/rdf-schema#comment> "A simulation route (AKA workroute) represents a sequence of process steps in manufacutring (mainly at wafer fab). This is a simulation entity and not a form of production/planning."@en .
<http://www.purl.org/i4go/variant-domain/operation/SimulationRoute> <http://www.w3.org/1999/02/22-rdf-syntax-ns#type> <http://www.w3.org/2002/07/owl#Class> .
<http://www.purl.org/i4go/variant-domain/operation/DepletionMode> <http://www.w3.org/2000/01/rdf-schema#label> "Depletion mode"@en .
<http://www.purl.org/i4go/variant-domain/operation/DepletionMode> <http://www.w3.org/2000/01/rdf-schema#comment> "A transistor that is normally closed (on), allowing current to pass, but is triggered to open (off) and impede current. Contrast with \"enhancement mode\", wherein the transistor is normally open (off), but is triggered to close (on)."@en .
<http://www.purl.org/i4go/variant-domain/operation/DepletionMode> <http://www.w3.org/2000/01/rdf-schema#subClassOf> <http://www.purl.org/i4go/variant-domain/operation/OperationMode> .
<http://www.purl.org/i4go/variant-domain/operation/DepletionMode> <http://www.w3.org/1999/02/22-rdf-syntax-ns#type> <http://www.w3.org/2002/07/owl#Class> .
<http://www.w3.org/ns/ssn/systems/hasOperatingProperty> <http://www.w3.org/2000/01/rdf-schema#label> "has operating property"@en .
<http://www.w3.org/ns/ssn/systems/hasOperatingProperty> <http://www.w3.org/2000/01/rdf-schema#comment> "Relation from an OperatingRange of a System to an OperatingProperty describing the operating range of the System."@en .
<http://www.w3.org/ns/ssn/systems/hasOperatingProperty> <http://www.w3.org/2000/01/rdf-schema#subPropertyOf> <http://www.w3.org/2002/07/owl#topObjectProperty> .
<http://www.w3.org/ns/ssn/systems/hasOperatingProperty> <http://www.w3.org/1999/02/22-rdf-syntax-ns#type> <http://www.w3.org/2002/07/owl#ObjectProperty> .
<http://www.w3id.org/ecsel-dr-SO#hasProcessingTimeDistribution> <http://www.w3.org/2000/01/rdf-schema#label> "has processing time distribution"@en .
<http://www.w3id.org/ecsel-dr-SO#hasProcessingTimeDistribution> <http://www.w3.org/2000/01/rdf-schema#range> <http://www.w3.org/2001/XMLSchema#string> .
<http://www.w3id.org/ecsel-dr-SO#hasProcessingTimeDistribution> <http://www.w3.org/2000/01/rdf-schema#domain> <http://www.w3id.org/ecsel-dr-SO#Operation> .
<http://www.w3id.org/ecsel-dr-SO#hasProcessingTimeDistribution> <http://www.w3.org/2000/01/rdf-schema#subPropertyOf> <http://www.w3.org/2002/07/owl#topDataProperty> .
<http://www.w3id.org/ecsel-dr-SO#hasProcessingTimeDistribution> <http://www.w3.org/1999/02/22-rdf-syntax-ns#type> <http://www.w3.org/2002/07/owl#DatatypeProperty> .
_:A6b5d418bX3aX17a61612d50X3aXX2dX7ff4 <http://www.w3.org/1999/02/22-rdf-syntax-ns#rest> <http://www.w3.org/1999/02/22-rdf-syntax-ns#nil> .
_:A6b5d418bX3aX17a61612d50X3aXX2dX7ff4 <http://www.w3.org/1999/02/22-rdf-syntax-ns#first> <http://www.w3id.org/ecsel-dr-SO#Operation> .
<http://www.w3id.org/ecsel-dr-SO#hasWorkshop> <http://www.w3.org/2000/01/rdf-schema#label> "has workshop"@en .
<http://www.w3id.org/ecsel-dr-SO#hasWorkshop> <http://www.w3.org/2000/01/rdf-schema#comment> "This class is used to relate operations with their related working structures."@en .
<http://www.w3id.org/ecsel-dr-SO#hasWorkshop> <http://www.w3.org/2000/01/rdf-schema#range> <http://www.w3id.org/ecsel-dr-SO#Workshop> .
<http://www.w3id.org/ecsel-dr-SO#hasWorkshop> <http://www.w3.org/2000/01/rdf-schema#domain> <http://www.w3id.org/ecsel-dr-SO#Operation> .
<http://www.w3id.org/ecsel-dr-SO#hasWorkshop> <http://www.w3.org/2000/01/rdf-schema#subPropertyOf> <http://www.w3.org/2002/07/owl#topObjectProperty> .
<http://www.w3id.org/ecsel-dr-SO#hasWorkshop> <http://www.w3.org/1999/02/22-rdf-syntax-ns#type> <http://www.w3.org/2002/07/owl#ObjectProperty> .
<http://www.purl.org/i4go/variant-domain/operation/DemandSnapshot> <http://www.w3.org/2000/01/rdf-schema#label> "Demand snapshot"@en .
<http://www.purl.org/i4go/variant-domain/operation/DemandSnapshot> <http://www.w3.org/2000/01/rdf-schema#comment> "The \u201CDemand\u201D entity stores redundant demand at every product level."@en .
<http://www.purl.org/i4go/variant-domain/operation/DemandSnapshot> <http://www.w3.org/1999/02/22-rdf-syntax-ns#type> <http://www.w3.org/2002/07/owl#Class> .
<http://www.purl.org/i4go/variant-domain/operation/LotSize> <http://www.w3.org/2000/01/rdf-schema#label> "Lot size"@en .
<http://www.purl.org/i4go/variant-domain/operation/LotSize> <http://www.w3.org/2000/01/rdf-schema#comment> "A measure or quantity increment acceptable to or specified by the party offering to buy or sell. Used also as an alternative term for lot quantity."@en .
<http://www.purl.org/i4go/variant-domain/operation/LotSize> <http://www.w3.org/1999/02/22-rdf-syntax-ns#type> <http://www.w3.org/2002/07/owl#Class> .
<http://www.w3id.org/ecsel-dr-SO#hasRouteName> <http://www.w3.org/2000/01/rdf-schema#label> "has route name"@en .
<http://www.w3id.org/ecsel-dr-SO#hasRouteName> <http://www.w3.org/2000/01/rdf-schema#comment> "Name of route (usually equals product names requiring the route)."@en .
<http://www.w3id.org/ecsel-dr-SO#hasRouteName> <http://www.w3.org/2000/01/rdf-schema#range> <http://www.w3.org/2001/XMLSchema#string> .
<http://www.w3id.org/ecsel-dr-SO#hasRouteName> <http://www.w3.org/2000/01/rdf-schema#domain> <http://www.w3id.org/ecsel-dr-SO#Route> .
<http://www.w3id.org/ecsel-dr-SO#hasRouteName> <http://www.w3.org/2000/01/rdf-schema#subPropertyOf> <http://www.w3.org/2002/07/owl#topDataProperty> .
<http://www.w3id.org/ecsel-dr-SO#hasRouteName> <http://www.w3.org/1999/02/22-rdf-syntax-ns#type> <http://www.w3.org/2002/07/owl#DatatypeProperty> .
_:A6b5d418bX3aX17a61612d50X3aXX2dX7ffa <http://www.w3.org/1999/02/22-rdf-syntax-ns#rest> <http://www.w3.org/1999/02/22-rdf-syntax-ns#nil> .
_:A6b5d418bX3aX17a61612d50X3aXX2dX7ffa <http://www.w3.org/1999/02/22-rdf-syntax-ns#first> <http://www.w3id.org/ecsel-dr-SO#Operation> .
<http://www.purl.org/i4go/variant-domain/operation/ProductionRequests> <http://www.w3.org/2000/01/rdf-schema#label> "Production requests"@en .
<http://www.purl.org/i4go/variant-domain/operation/ProductionRequests> <http://www.w3.org/2000/01/rdf-schema#comment> "Production requests definte what the facilities need to produce when and in what quantity."@en .
<http://www.purl.org/i4go/variant-domain/operation/ProductionRequests> <http://www.w3.org/1999/02/22-rdf-syntax-ns#type> <http://www.w3.org/2002/07/owl#Class> .
<http://www.w3id.org/ecsel-dr-SO#hasMeanTimeToRepairDistribution> <http://www.w3.org/2000/01/rdf-schema#label> "has mean time to repair distribution"@en .
<http://www.w3id.org/ecsel-dr-SO#hasMeanTimeToRepairDistribution> <http://www.w3.org/2000/01/rdf-schema#range> <http://www.w3.org/2001/XMLSchema#string> .
<http://www.w3id.org/ecsel-dr-SO#hasMeanTimeToRepairDistribution> <http://www.w3.org/2000/01/rdf-schema#domain> <http://www.purl.org/i4go/variant-domain/operation/EventCalendar> .
<http://www.w3id.org/ecsel-dr-SO#hasMeanTimeToRepairDistribution> <http://www.w3.org/2000/01/rdf-schema#subPropertyOf> <http://www.w3.org/2002/07/owl#topDataProperty> .
<http://www.w3id.org/ecsel-dr-SO#hasMeanTimeToRepairDistribution> <http://www.w3.org/1999/02/22-rdf-syntax-ns#type> <http://www.w3.org/2002/07/owl#DatatypeProperty> .
<http://www.purl.org/i4go/variant-domain/operation/Off-StateRegion> <http://www.w3.org/2000/01/rdf-schema#label> "Off-state region"@en .
<http://www.purl.org/i4go/variant-domain/operation/Off-StateRegion> <http://www.w3.org/2000/01/rdf-schema#subClassOf> <http://www.purl.org/i4go/variant-domain/operation/RegionOfOperation> .
<http://www.purl.org/i4go/variant-domain/operation/Off-StateRegion> <http://www.w3.org/1999/02/22-rdf-syntax-ns#type> <http://www.w3.org/2002/07/owl#Class> .
_:A6b5d418bX3aX17a61612d50X3aXX2dX7ff9 <http://www.w3.org/2002/07/owl#unionOf> _:A6b5d418bX3aX17a61612d50X3aXX2dX7ff8 .
_:A6b5d418bX3aX17a61612d50X3aXX2dX7ff9 <http://www.w3.org/1999/02/22-rdf-syntax-ns#type> <http://www.w3.org/2002/07/owl#Class> .
<http://www.purl.org/i4go/variant-domain/operation/Triode/ConstantResistanceRegion> <http://www.w3.org/2000/01/rdf-schema#label> "Cosntant resistance region"@en .
<http://www.purl.org/i4go/variant-domain/operation/Triode/ConstantResistanceRegion> <http://www.w3.org/2000/01/rdf-schema#subClassOf> <http://www.purl.org/i4go/variant-domain/operation/On-StateRegion> .
<http://www.purl.org/i4go/variant-domain/operation/Triode/ConstantResistanceRegion> <http://www.w3.org/1999/02/22-rdf-syntax-ns#type> <http://www.w3.org/2002/07/owl#Class> .
<http://www.w3id.org/ecsel-dr-SO#hasPart> <http://www.w3.org/2000/01/rdf-schema#label> "has part"@en .
<http://www.w3id.org/ecsel-dr-SO#hasPart> <http://www.w3.org/2000/01/rdf-schema#range> <http://www.purl.org/i4go/variant-domain/operation/SimulationPart> .
<http://www.w3id.org/ecsel-dr-SO#hasPart> <http://www.w3.org/2000/01/rdf-schema#domain> <http://www.purl.org/i4go/variant-domain/operation/SimulationRoute> .
<http://www.w3id.org/ecsel-dr-SO#hasPart> <http://www.w3.org/2000/01/rdf-schema#subPropertyOf> <http://www.w3.org/2002/07/owl#topObjectProperty> .
<http://www.w3id.org/ecsel-dr-SO#hasPart> <http://www.w3.org/1999/02/22-rdf-syntax-ns#type> <http://www.w3.org/2002/07/owl#ObjectProperty> .
<http://www.purl.org/i4go/variant-domain/operation/ThresholdVoltage> <http://www.w3.org/2000/01/rdf-schema#label> "Threshold voltage"@en .
<http://www.purl.org/i4go/variant-domain/operation/ThresholdVoltage> <http://www.w3.org/2000/01/rdf-schema#comment> "The threshold voltage, commonly abbreviated as Vth, of a field-effect transistor (FET) is the minimum gate-to-source voltage VGS (th) that is needed to create a conducting path between the source and drain terminals. It is an important scaling factor to maintain power efficiency."@en .
<http://www.purl.org/i4go/variant-domain/operation/ThresholdVoltage> <http://www.w3.org/2000/01/rdf-schema#subClassOf> <http://www.purl.org/i4go/variant-domain/operation/OperatingProperty> .
<http://www.purl.org/i4go/variant-domain/operation/ThresholdVoltage> <http://www.w3.org/1999/02/22-rdf-syntax-ns#type> <http://www.w3.org/2002/07/owl#Class> .
_:A6b5d418bX3aX17a61612d50X3aXX2dX7ff3 <http://www.w3.org/2002/07/owl#unionOf> _:A6b5d418bX3aX17a61612d50X3aXX2dX7ff2 .
_:A6b5d418bX3aX17a61612d50X3aXX2dX7ff3 <http://www.w3.org/1999/02/22-rdf-syntax-ns#type> <http://www.w3.org/2002/07/owl#Class> .
<http://www.purl.org/i4go/variant-domain/operation/OperationMode> <http://www.w3.org/2000/01/rdf-schema#label> "Operation mode"@en .
<http://www.purl.org/i4go/variant-domain/operation/OperationMode> <http://www.w3.org/2000/01/rdf-schema#comment> "An operational situation/configuration of a system characterized by its active functions. Inside an operational mode the system can perform specific operational scenarios, and so activate the corresponding functions."@en .
<http://www.purl.org/i4go/variant-domain/operation/OperationMode> <http://www.w3.org/1999/02/22-rdf-syntax-ns#type> <http://www.w3.org/2002/07/owl#Class> .
<http://www.w3id.org/ecsel-dr-SO#hasUnit> <http://www.w3.org/2000/01/rdf-schema#label> "has unit"@en .
<http://www.w3id.org/ecsel-dr-SO#hasUnit> <http://www.w3.org/2000/01/rdf-schema#comment> "Unit, added due to data import"@en .
<http://www.w3id.org/ecsel-dr-SO#hasUnit> <http://www.w3.org/2000/01/rdf-schema#range> <http://www.w3.org/2001/XMLSchema#string> .
<http://www.w3id.org/ecsel-dr-SO#hasUnit> <http://www.w3.org/2000/01/rdf-schema#domain> <http://www.w3id.org/ecsel-dr-SO#Operation> .
<http://www.w3id.org/ecsel-dr-SO#hasUnit> <http://www.w3.org/2000/01/rdf-schema#subPropertyOf> <http://www.w3.org/2002/07/owl#topDataProperty> .
<http://www.w3id.org/ecsel-dr-SO#hasUnit> <http://www.w3.org/1999/02/22-rdf-syntax-ns#type> <http://www.w3.org/2002/07/owl#DatatypeProperty> .
<http://www.w3id.org/ecsel-dr-SO#hasOperationName> <http://www.w3.org/2000/01/rdf-schema#label> "has operation name"@en .
<http://www.w3id.org/ecsel-dr-SO#hasOperationName> <http://www.w3.org/2000/01/rdf-schema#comment> "Name of the operation."@en .
<http://www.w3id.org/ecsel-dr-SO#hasOperationName> <http://www.w3.org/2000/01/rdf-schema#range> <http://www.w3.org/2001/XMLSchema#string> .
<http://www.w3id.org/ecsel-dr-SO#hasOperationName> <http://www.w3.org/2000/01/rdf-schema#domain> <http://www.w3id.org/ecsel-dr-SO#Operation> .
<http://www.w3id.org/ecsel-dr-SO#hasOperationName> <http://www.w3.org/2000/01/rdf-schema#subPropertyOf> <http://www.w3.org/2002/07/owl#topDataProperty> .
<http://www.w3id.org/ecsel-dr-SO#hasOperationName> <http://www.w3.org/1999/02/22-rdf-syntax-ns#type> <http://www.w3.org/2002/07/owl#DatatypeProperty> .
<http://www.w3id.org/ecsel-dr-SO#hasEquipment> <http://www.w3.org/2000/01/rdf-schema#label> "has equipment"@en .
<http://www.w3id.org/ecsel-dr-SO#hasEquipment> <http://www.w3.org/2000/01/rdf-schema#comment> "Property used to relate operations with the equipment that perform them."@en .
<http://www.w3id.org/ecsel-dr-SO#hasEquipment> <http://www.w3.org/2000/01/rdf-schema#range> <http://www.w3id.org/ecsel-dr-SO#Equipment> .
<http://www.w3id.org/ecsel-dr-SO#hasEquipment> <http://www.w3.org/2000/01/rdf-schema#domain> <http://www.w3id.org/ecsel-dr-SO#Operation> .
<http://www.w3id.org/ecsel-dr-SO#hasEquipment> <http://www.w3.org/2002/07/owl#inverseOf> <http://www.w3id.org/ecsel-dr-SO#isEquipmentOf> .
<http://www.w3id.org/ecsel-dr-SO#hasEquipment> <http://www.w3.org/2000/01/rdf-schema#subPropertyOf> <http://www.w3.org/2002/07/owl#topObjectProperty> .
<http://www.w3id.org/ecsel-dr-SO#hasEquipment> <http://www.w3.org/1999/02/22-rdf-syntax-ns#type> <http://www.w3.org/2002/07/owl#ObjectProperty> .
<http://www.w3id.org/ecsel-dr-SO#hasTimeConstraints> <http://www.w3.org/2000/01/rdf-schema#label> "has time constraints"@en .
<http://www.w3id.org/ecsel-dr-SO#hasTimeConstraints> <http://www.w3.org/2000/01/rdf-schema#comment> "This class is used to relate operations with their time constraints."@en .
<http://www.w3id.org/ecsel-dr-SO#hasTimeConstraints> <http://www.w3.org/2000/01/rdf-schema#range> <http://www.purl.org/i4go/variant-domain/operation/TimeConstraints> .
<http://www.w3id.org/ecsel-dr-SO#hasTimeConstraints> <http://www.w3.org/2000/01/rdf-schema#domain> <http://www.w3id.org/ecsel-dr-SO#Operation> .
<http://www.w3id.org/ecsel-dr-SO#hasTimeConstraints> <http://www.w3.org/2000/01/rdf-schema#subPropertyOf> <http://www.w3.org/2002/07/owl#topObjectProperty> .
<http://www.w3id.org/ecsel-dr-SO#hasTimeConstraints> <http://www.w3.org/1999/02/22-rdf-syntax-ns#type> <http://www.w3.org/2002/07/owl#ObjectProperty> .
<http://www.purl.org/i4go/variant-domain/operation/EventCalendar> <http://www.w3.org/2000/01/rdf-schema#label> "Event calendar"@en .
<http://www.purl.org/i4go/variant-domain/operation/EventCalendar> <http://www.w3.org/2000/01/rdf-schema#comment> "An event calendar is an organized way to show the upcoming events based on calendar dates."@en .
<http://www.purl.org/i4go/variant-domain/operation/EventCalendar> <http://www.w3.org/1999/02/22-rdf-syntax-ns#type> <http://www.w3.org/2002/07/owl#Class> .
<http://www.purl.org/i4go/variant-domain/operation/WetEtching> <http://www.w3.org/2000/01/rdf-schema#label> "Wet etching"@en .
<http://www.purl.org/i4go/variant-domain/operation/WetEtching> <http://www.w3.org/2000/01/rdf-schema#comment> "Wet Etching is the process of removing material-etching, through the use of chemical activity."@en .
<http://www.purl.org/i4go/variant-domain/operation/WetEtching> <http://www.w3.org/2000/01/rdf-schema#subClassOf> <http://www.w3id.org/ecsel-dr-SO#Workshop> .
<http://www.purl.org/i4go/variant-domain/operation/WetEtching> <http://www.w3.org/1999/02/22-rdf-syntax-ns#type> <http://www.w3.org/2002/07/owl#Class> .
<http://www.w3id.org/ecsel-dr-SO#hasReworkProbabilityLots> <http://www.w3.org/2000/01/rdf-schema#label> "has rework probability lots"@en .
<http://www.w3id.org/ecsel-dr-SO#hasReworkProbabilityLots> <http://www.w3.org/2000/01/rdf-schema#comment> "Operation: Probability of rework-tested full lots to be reworked."@en .
<http://www.w3id.org/ecsel-dr-SO#hasReworkProbabilityLots> <http://www.w3.org/2000/01/rdf-schema#range> <http://www.w3.org/2001/XMLSchema#double> .
<http://www.w3id.org/ecsel-dr-SO#hasReworkProbabilityLots> <http://www.w3.org/2000/01/rdf-schema#domain> <http://www.w3id.org/ecsel-dr-SO#Operation> .
<http://www.w3id.org/ecsel-dr-SO#hasReworkProbabilityLots> <http://www.w3.org/2000/01/rdf-schema#subPropertyOf> <http://www.w3.org/2002/07/owl#topDataProperty> .
<http://www.w3id.org/ecsel-dr-SO#hasReworkProbabilityLots> <http://www.w3.org/1999/02/22-rdf-syntax-ns#type> <http://www.w3.org/2002/07/owl#DatatypeProperty> .
<http://www.w3id.org/ecsel-dr-SO#hasEquipmentGroup> <http://www.w3.org/2000/01/rdf-schema#label> "has equipment group"@en .
<http://www.w3id.org/ecsel-dr-SO#hasEquipmentGroup> <http://www.w3.org/2000/01/rdf-schema#comment> "This property is used to relate operations with the equipment groups that perform them."@en .
<http://www.w3id.org/ecsel-dr-SO#hasEquipmentGroup> <http://www.w3.org/2000/01/rdf-schema#range> <http://www.purl.org/i4go/common-domain/equipment/EquipmentGroup> .
<http://www.w3id.org/ecsel-dr-SO#hasEquipmentGroup> <http://www.w3.org/2000/01/rdf-schema#domain> _:A6b5d418bX3aX17a61612d50X3aXX2dX7ff9 .
<http://www.w3id.org/ecsel-dr-SO#hasEquipmentGroup> <http://www.w3.org/2000/01/rdf-schema#subPropertyOf> <http://www.w3.org/2002/07/owl#topObjectProperty> .
<http://www.w3id.org/ecsel-dr-SO#hasEquipmentGroup> <http://www.w3.org/1999/02/22-rdf-syntax-ns#type> <http://www.w3.org/2002/07/owl#ObjectProperty> .
<http://www.w3id.org/ecsel-dr-SO#Route> <http://www.w3.org/2000/01/rdf-schema#label> "Route"@en .
<http://www.w3id.org/ecsel-dr-SO#Route> <http://www.w3.org/2000/01/rdf-schema#comment> "The master entity \u201CRoute\u201D describes the structure of a workflow out of operations. Every product uses a specific route in its value stream, i.e. the complete sequence of operations with all mandatory and optional operations necessary to complete the product. A route makes use of the single operations. (workflow descriptive master entity)."@en .
<http://www.w3id.org/ecsel-dr-SO#Route> <http://www.w3.org/1999/02/22-rdf-syntax-ns#type> <http://www.w3.org/2002/07/owl#Class> .
<http://www.w3id.org/ecsel-dr-SO#hasPTimePerUnit> <http://www.w3.org/2000/01/rdf-schema#label> "has P time per unit"@en .
<http://www.w3id.org/ecsel-dr-SO#hasPTimePerUnit> <http://www.w3.org/2000/01/rdf-schema#comment> "Length of, or element of the length of, a temporal extent expressed in seconds"@en .
<http://www.w3id.org/ecsel-dr-SO#hasPTimePerUnit> <http://www.w3.org/2000/01/rdf-schema#range> <http://www.w3.org/2001/XMLSchema#decimal> .
<http://www.w3id.org/ecsel-dr-SO#hasPTimePerUnit> <http://www.w3.org/2000/01/rdf-schema#domain> <http://www.w3id.org/ecsel-dr-SO#Operation> .
<http://www.w3id.org/ecsel-dr-SO#hasPTimePerUnit> <http://www.w3.org/2000/01/rdf-schema#subPropertyOf> <http://www.w3.org/2002/07/owl#topDataProperty> .
<http://www.w3id.org/ecsel-dr-SO#hasPTimePerUnit> <http://www.w3.org/1999/02/22-rdf-syntax-ns#type> <http://www.w3.org/2002/07/owl#DatatypeProperty> .
_:A6b5d418bX3aX17a61612d50X3aXX2dX7ff8 <http://www.w3.org/1999/02/22-rdf-syntax-ns#rest> _:A6b5d418bX3aX17a61612d50X3aXX2dX7ff7 .
_:A6b5d418bX3aX17a61612d50X3aXX2dX7ff8 <http://www.w3.org/1999/02/22-rdf-syntax-ns#first> <http://www.purl.org/i4go/variant-domain/operation/EventCalendar> .
<http://www.w3id.org/ecsel-dr-SO#hasSequenceNumber> <http://www.w3.org/2000/01/rdf-schema#label> "has sequence number"@en .
<http://www.w3id.org/ecsel-dr-SO#hasSequenceNumber> <http://www.w3.org/2000/01/rdf-schema#comment> "Lot Event: FK; Sequential number of the operation lot has entered"@en .
<http://www.w3id.org/ecsel-dr-SO#hasSequenceNumber> <http://www.w3.org/2000/01/rdf-schema#range> <http://www.w3.org/2001/XMLSchema#integer> .
<http://www.w3id.org/ecsel-dr-SO#hasSequenceNumber> <http://www.w3.org/2000/01/rdf-schema#domain> <http://www.w3id.org/ecsel-dr-SO#Route> .
<http://www.w3id.org/ecsel-dr-SO#hasSequenceNumber> <http://www.w3.org/2000/01/rdf-schema#subPropertyOf> <http://www.w3.org/2002/07/owl#topDataProperty> .
<http://www.w3id.org/ecsel-dr-SO#hasSequenceNumber> <http://www.w3.org/1999/02/22-rdf-syntax-ns#type> <http://www.w3.org/2002/07/owl#DatatypeProperty> .
<http://www.w3id.org/ecsel-dr-SO#hasSamplingRate> <http://www.w3.org/2000/01/rdf-schema#label> "has sampling rate"@en .
<http://www.w3id.org/ecsel-dr-SO#hasSamplingRate> <http://www.w3.org/2000/01/rdf-schema#comment> "Sampling Rate: Execution rate of operation If operation is mandatory sampling rate is 1 (1- sampling rate = skipping rate of optional operation)"@en .
<http://www.w3id.org/ecsel-dr-SO#hasSamplingRate> <http://www.w3.org/2000/01/rdf-schema#range> <http://www.w3.org/2001/XMLSchema#double> .
<http://www.w3id.org/ecsel-dr-SO#hasSamplingRate> <http://www.w3.org/2000/01/rdf-schema#domain> <http://www.w3id.org/ecsel-dr-SO#Operation> .
<http://www.w3id.org/ecsel-dr-SO#hasSamplingRate> <http://www.w3.org/2000/01/rdf-schema#subPropertyOf> <http://www.w3.org/2002/07/owl#topDataProperty> .
<http://www.w3id.org/ecsel-dr-SO#hasSamplingRate> <http://www.w3.org/1999/02/22-rdf-syntax-ns#type> <http://www.w3.org/2002/07/owl#DatatypeProperty> .
<http://www.w3id.org/ecsel-dr-SO#hasScrappingTest> <http://www.w3.org/2000/01/rdf-schema#label> "has scrapping test"@en .
<http://www.w3id.org/ecsel-dr-SO#hasScrappingTest> <http://www.w3.org/2000/01/rdf-schema#comment> "Operation: Are the processed lots tested for scrapping?"@en .
<http://www.w3id.org/ecsel-dr-SO#hasScrappingTest> <http://www.w3.org/2000/01/rdf-schema#range> <http://www.w3.org/2001/XMLSchema#boolean> .
<http://www.w3id.org/ecsel-dr-SO#hasScrappingTest> <http://www.w3.org/2000/01/rdf-schema#domain> <http://www.w3id.org/ecsel-dr-SO#Operation> .
<http://www.w3id.org/ecsel-dr-SO#hasScrappingTest> <http://www.w3.org/2000/01/rdf-schema#subPropertyOf> <http://www.w3.org/2002/07/owl#topDataProperty> .
<http://www.w3id.org/ecsel-dr-SO#hasScrappingTest> <http://www.w3.org/1999/02/22-rdf-syntax-ns#type> <http://www.w3.org/2002/07/owl#DatatypeProperty> .
<http://www.w3id.org/ecsel-dr-SO#hasMeanTimeToFailureDistribution> <http://www.w3.org/2000/01/rdf-schema#label> "has mean time to failure distribution"@en .
<http://www.w3id.org/ecsel-dr-SO#hasMeanTimeToFailureDistribution> <http://www.w3.org/2000/01/rdf-schema#range> <http://www.w3.org/2001/XMLSchema#string> .
<http://www.w3id.org/ecsel-dr-SO#hasMeanTimeToFailureDistribution> <http://www.w3.org/2000/01/rdf-schema#domain> <http://www.purl.org/i4go/variant-domain/operation/EventCalendar> .
<http://www.w3id.org/ecsel-dr-SO#hasMeanTimeToFailureDistribution> <http://www.w3.org/2000/01/rdf-schema#subPropertyOf> <http://www.w3.org/2002/07/owl#topDataProperty> .
<http://www.w3id.org/ecsel-dr-SO#hasMeanTimeToFailureDistribution> <http://www.w3.org/1999/02/22-rdf-syntax-ns#type> <http://www.w3.org/2002/07/owl#DatatypeProperty> .
<http://www.w3id.org/ecsel-dr-SO#hasReworkTest> <http://www.w3.org/2000/01/rdf-schema#label> "has rework test"@en .
<http://www.w3id.org/ecsel-dr-SO#hasReworkTest> <http://www.w3.org/2000/01/rdf-schema#comment> "Operation: Are the processed lots tested for rework?"@en .
<http://www.w3id.org/ecsel-dr-SO#hasReworkTest> <http://www.w3.org/2000/01/rdf-schema#range> <http://www.w3.org/2001/XMLSchema#boolean> .
<http://www.w3id.org/ecsel-dr-SO#hasReworkTest> <http://www.w3.org/2000/01/rdf-schema#domain> <http://www.w3id.org/ecsel-dr-SO#Operation> .
<http://www.w3id.org/ecsel-dr-SO#hasReworkTest> <http://www.w3.org/2000/01/rdf-schema#subPropertyOf> <http://www.w3.org/2002/07/owl#topDataProperty> .
<http://www.w3id.org/ecsel-dr-SO#hasReworkTest> <http://www.w3.org/1999/02/22-rdf-syntax-ns#type> <http://www.w3.org/2002/07/owl#DatatypeProperty> .
<http://www.w3.org/ns/ssn/Property> <http://www.w3.org/1999/02/22-rdf-syntax-ns#type> <http://www.w3.org/2002/07/owl#Class> .
_:A6b5d418bX3aX17a61612d50X3aXX2dX7ff2 <http://www.w3.org/1999/02/22-rdf-syntax-ns#rest> _:A6b5d418bX3aX17a61612d50X3aXX2dX7ff1 .
_:A6b5d418bX3aX17a61612d50X3aXX2dX7ff2 <http://www.w3.org/1999/02/22-rdf-syntax-ns#first> <http://www.purl.org/i4go/common-domain/equipment/EquipmentGroup> .
<http://www.purl.org/i4go/variant-domain/operation> <http://purl.org/dc/terms/issued> "2021-05-03"@en .
<http://www.purl.org/i4go/variant-domain/operation> <http://www.w3.org/2000/01/rdf-schema#comment> "The 'Operation' ontology module represents information about operations: combination of activities necessary to permit an installation to function. The represented operations include switching, controlling, monitoring and maintenance as well as any work activities."@en .
<http://www.purl.org/i4go/variant-domain/operation> <http://creativecommons.org/ns#license> "https://creativecommons.org/licenses/by-nc/4.0/"@en .
<http://www.purl.org/i4go/variant-domain/operation> <http://purl.org/dc/terms/creator> "Javier Cuenca <mailto:jcuenca@mondragon.edu>\nFelix Larrinaga <mailto:flarrinaga@mondragon.edu>"@en .
<http://www.purl.org/i4go/variant-domain/operation> <http://www.w3.org/2002/07/owl#versionInfo> "1.0"@en .
<http://www.purl.org/i4go/variant-domain/operation> <http://purl.org/dc/elements/1.1/title> "Operation ontology"@en .
<http://www.purl.org/i4go/variant-domain/operation> <http://www.w3.org/2002/07/owl#imports> <http://www.purl.org/i4go/common-domain/equipment> .
<http://www.purl.org/i4go/variant-domain/operation> <http://www.w3.org/1999/02/22-rdf-syntax-ns#type> <http://www.w3.org/2002/07/owl#Ontology> .
<http://www.purl.org/i4go/variant-domain/operation/On-StateRegion> <http://www.w3.org/2000/01/rdf-schema#label> "On-state region"@en .
<http://www.purl.org/i4go/variant-domain/operation/On-StateRegion> <http://www.w3.org/2000/01/rdf-schema#subClassOf> <http://www.purl.org/i4go/variant-domain/operation/RegionOfOperation> .
<http://www.purl.org/i4go/variant-domain/operation/On-StateRegion> <http://www.w3.org/1999/02/22-rdf-syntax-ns#type> <http://www.w3.org/2002/07/owl#Class> .
<http://www.w3id.org/ecsel-dr-SO#hasOperationID> <http://www.w3.org/2000/01/rdf-schema#label> "has operation ID"@en .
<http://www.w3id.org/ecsel-dr-SO#hasOperationID> <http://www.w3.org/2000/01/rdf-schema#comment> "Operation identifier"@en .
<http://www.w3id.org/ecsel-dr-SO#hasOperationID> <http://www.w3.org/2000/01/rdf-schema#range> <http://www.w3.org/2001/XMLSchema#string> .
<http://www.w3id.org/ecsel-dr-SO#hasOperationID> <http://www.w3.org/2000/01/rdf-schema#domain> <http://www.w3id.org/ecsel-dr-SO#Route> .
<http://www.w3id.org/ecsel-dr-SO#hasOperationID> <http://www.w3.org/2000/01/rdf-schema#domain> <http://www.w3id.org/ecsel-dr-SO#Operation> .
<http://www.w3id.org/ecsel-dr-SO#hasOperationID> <http://www.w3.org/2000/01/rdf-schema#subPropertyOf> <http://www.w3.org/2002/07/owl#topDataProperty> .
<http://www.w3id.org/ecsel-dr-SO#hasOperationID> <http://www.w3.org/1999/02/22-rdf-syntax-ns#type> <http://www.w3.org/2002/07/owl#DatatypeProperty> .
<http://www.purl.org/i4go/variant-domain/operation/ProductLevel> <http://www.w3.org/2000/01/rdf-schema#label> "Product level"@en .
<http://www.purl.org/i4go/variant-domain/operation/ProductLevel> <http://www.w3.org/2000/01/rdf-schema#comment> "In the \"product level\" entity, the aggregation of elements enables the grouping of products and defines the relationship between products and groups at different hierarchy levels. This supports planning, logistics, modeling, forecasting and reporting."@en .
<http://www.purl.org/i4go/variant-domain/operation/ProductLevel> <http://www.w3.org/1999/02/22-rdf-syntax-ns#type> <http://www.w3.org/2002/07/owl#Class> .
<http://www.w3id.org/ecsel-dr-SO#hasScrappingProbabilityLots> <http://www.w3.org/2000/01/rdf-schema#label> "has scrapping probability lots"@en .
<http://www.w3id.org/ecsel-dr-SO#hasScrappingProbabilityLots> <http://www.w3.org/2000/01/rdf-schema#comment> "Operation: Probability of scrapping-tested full lots to be scrapped."@en .
<http://www.w3id.org/ecsel-dr-SO#hasScrappingProbabilityLots> <http://www.w3.org/2000/01/rdf-schema#range> <http://www.w3.org/2001/XMLSchema#double> .
<http://www.w3id.org/ecsel-dr-SO#hasScrappingProbabilityLots> <http://www.w3.org/2000/01/rdf-schema#domain> <http://www.w3id.org/ecsel-dr-SO#Operation> .
<http://www.w3id.org/ecsel-dr-SO#hasScrappingProbabilityLots> <http://www.w3.org/2000/01/rdf-schema#subPropertyOf> <http://www.w3.org/2002/07/owl#topDataProperty> .
<http://www.w3id.org/ecsel-dr-SO#hasScrappingProbabilityLots> <http://www.w3.org/1999/02/22-rdf-syntax-ns#type> <http://www.w3.org/2002/07/owl#DatatypeProperty> .
<http://www.w3id.org/ecsel-dr-SO#Technology> <http://www.w3.org/2000/01/rdf-schema#label> "Technology"@en .
<http://www.w3id.org/ecsel-dr-SO#Technology> <http://www.w3.org/2000/01/rdf-schema#comment> "A semiconductor technology is a set of equipment, processes, manufacturing techniques and the related methods and procedures to enable the design & production of components, sub-components and modules."@en .
<http://www.w3id.org/ecsel-dr-SO#Technology> <http://www.w3.org/1999/02/22-rdf-syntax-ns#type> <http://www.w3.org/2002/07/owl#Class> .
<http://www.w3id.org/ecsel-dr-SO#hasCapacityLoss> <http://www.w3.org/2000/01/rdf-schema#label> "has capacity loss"@en .
<http://www.w3id.org/ecsel-dr-SO#hasCapacityLoss> <http://www.w3.org/2000/01/rdf-schema#comment> "Calendar: Facility capacity loss in percent."@en .
<http://www.w3id.org/ecsel-dr-SO#hasCapacityLoss> <http://www.w3.org/2000/01/rdf-schema#range> <http://www.w3.org/2001/XMLSchema#double> .
<http://www.w3id.org/ecsel-dr-SO#hasCapacityLoss> <http://www.w3.org/2000/01/rdf-schema#domain> <http://www.purl.org/i4go/variant-domain/operation/EventCalendar> .
<http://www.w3id.org/ecsel-dr-SO#hasCapacityLoss> <http://www.w3.org/2000/01/rdf-schema#subPropertyOf> <http://www.w3.org/2002/07/owl#topDataProperty> .
<http://www.w3id.org/ecsel-dr-SO#hasCapacityLoss> <http://www.w3.org/1999/02/22-rdf-syntax-ns#type> <http://www.w3.org/2002/07/owl#DatatypeProperty> .
_:A6b5d418bX3aX17a61612d50X3aXX2dX7ff7 <http://www.w3.org/1999/02/22-rdf-syntax-ns#rest> <http://www.w3.org/1999/02/22-rdf-syntax-ns#nil> .
_:A6b5d418bX3aX17a61612d50X3aXX2dX7ff7 <http://www.w3.org/1999/02/22-rdf-syntax-ns#first> <http://www.w3id.org/ecsel-dr-SO#Operation> .
<http://www.w3id.org/ecsel-dr-SO#Deposition> <http://www.w3.org/2000/01/rdf-schema#label> "Deposition"@en .
<http://www.w3id.org/ecsel-dr-SO#Deposition> <http://www.w3.org/2000/01/rdf-schema#comment> "The deposition process, or chemical vapor deposition (CVD) is a process whereby a fiolm is deposited by reacting chemicals together in the gaseous or vapor phase to form a film. The gases or vapors utilized for CVD are compounds that contain the element to be deposited and that may be inducted to react with a substrate or other gas(es) to deposit a film. The CVD reactoin may be thermally activated, plasma induced, plasma enhanced CVD or activated by light in photon induced CVD."@en .
<http://www.w3id.org/ecsel-dr-SO#Deposition> <http://www.w3.org/2000/01/rdf-schema#subClassOf> <http://www.w3id.org/ecsel-dr-SO#Workshop> .
<http://www.w3id.org/ecsel-dr-SO#Deposition> <http://www.w3.org/1999/02/22-rdf-syntax-ns#type> <http://www.w3.org/2002/07/owl#Class> .
<http://www.w3id.org/ecsel-dr-SO#Sputtering> <http://www.w3.org/2000/01/rdf-schema#label> "Sputtering"@en .
<http://www.w3id.org/ecsel-dr-SO#Sputtering> <http://www.w3.org/2000/01/rdf-schema#comment> "The sputtering process, or physical vapor deposition (PVD) is the most used layering process today. Here gas atoms, mostly argon, strike out atoms from the cathode I an electric field which then form a thin film on the wafer surface."@en .
<http://www.w3id.org/ecsel-dr-SO#Sputtering> <http://www.w3.org/2000/01/rdf-schema#subClassOf> <http://www.w3id.org/ecsel-dr-SO#Workshop> .
<http://www.w3id.org/ecsel-dr-SO#Sputtering> <http://www.w3.org/1999/02/22-rdf-syntax-ns#type> <http://www.w3.org/2002/07/owl#Class> .
<http://www.w3id.org/ecsel-dr-SO#CurrentWIP> <http://www.w3.org/2000/01/rdf-schema#label> "Current WIP"@en .
<http://www.w3id.org/ecsel-dr-SO#CurrentWIP> <http://www.w3.org/2000/01/rdf-schema#comment> "\u201CCurrent WIP\u201D entity describes the actual material distribution in the supply chain."@en .
<http://www.w3id.org/ecsel-dr-SO#CurrentWIP> <http://www.w3.org/1999/02/22-rdf-syntax-ns#type> <http://www.w3.org/2002/07/owl#Class> .
<http://www.purl.org/i4go/variant-domain/operation/SwitchingFrequency> <http://www.w3.org/2000/01/rdf-schema#label> "Switching frequency"@en .
<http://www.purl.org/i4go/variant-domain/operation/SwitchingFrequency> <http://www.w3.org/2000/01/rdf-schema#comment> "In electronics, switching frequency refers to the rate at which an electronic switch performs its function."@en .
<http://www.purl.org/i4go/variant-domain/operation/SwitchingFrequency> <http://www.w3.org/2000/01/rdf-schema#subClassOf> <http://www.purl.org/i4go/variant-domain/operation/OperatingProperty> .
<http://www.purl.org/i4go/variant-domain/operation/SwitchingFrequency> <http://www.w3.org/1999/02/22-rdf-syntax-ns#type> <http://www.w3.org/2002/07/owl#Class> .
<http://www.w3.org/2002/07/owl#topDataProperty> <http://www.w3.org/2000/01/rdf-schema#range> <http://www.w3.org/2001/XMLSchema#double> .
<http://www.w3.org/2002/07/owl#topDataProperty> <http://www.w3.org/2000/01/rdf-schema#domain> <http://www.w3id.org/ecsel-dr-SO#Operation> .
<http://www.w3id.org/ecsel-dr-SO#hasMeanTimeToFailure> <http://www.w3.org/2000/01/rdf-schema#label> "has mean time to failure"@en .
<http://www.w3id.org/ecsel-dr-SO#hasMeanTimeToFailure> <http://www.w3.org/2000/01/rdf-schema#comment> "Length of, or element of the length of, a temporal extent expressed in seconds"@en .
<http://www.w3id.org/ecsel-dr-SO#hasMeanTimeToFailure> <http://www.w3.org/2000/01/rdf-schema#range> <http://www.w3.org/2001/XMLSchema#decimal> .
<http://www.w3id.org/ecsel-dr-SO#hasMeanTimeToFailure> <http://www.w3.org/2000/01/rdf-schema#domain> <http://www.purl.org/i4go/variant-domain/operation/EventCalendar> .
<http://www.w3id.org/ecsel-dr-SO#hasMeanTimeToFailure> <http://www.w3.org/2000/01/rdf-schema#subPropertyOf> <http://www.w3.org/2002/07/owl#topDataProperty> .
<http://www.w3id.org/ecsel-dr-SO#hasMeanTimeToFailure> <http://www.w3.org/1999/02/22-rdf-syntax-ns#type> <http://www.w3.org/2002/07/owl#DatatypeProperty> .
<http://www.w3id.org/ecsel-dr-SO#Lithography> <http://www.w3.org/2000/01/rdf-schema#label> "Lithography"@en .
<http://www.w3id.org/ecsel-dr-SO#Lithography> <http://www.w3.org/2000/01/rdf-schema#comment> "The lithography process is the key process in frontend. This consists of the following steps: a photo resisting layer is spun on a wafer, then exposed through the mask, then developed, then showing the effect on the open places, and then final deletion of the photo resisting material leaves only the remaining structure on the water. after some time for deposition, these steps are repeated up to 35 times."@en .
<http://www.w3id.org/ecsel-dr-SO#Lithography> <http://www.w3.org/2000/01/rdf-schema#subClassOf> <http://www.w3id.org/ecsel-dr-SO#Workshop> .
<http://www.w3id.org/ecsel-dr-SO#Lithography> <http://www.w3.org/1999/02/22-rdf-syntax-ns#type> <http://www.w3.org/2002/07/owl#Class> .
_:A6b5d418bX3aX17a61612d50X3aXX2dX7ff1 <http://www.w3.org/1999/02/22-rdf-syntax-ns#rest> _:A6b5d418bX3aX17a61612d50X3aXX2dX7ff0 .
_:A6b5d418bX3aX17a61612d50X3aXX2dX7ff1 <http://www.w3.org/1999/02/22-rdf-syntax-ns#first> <http://www.purl.org/i4go/variant-domain/operation/DemandSnapshot> .
<http://www.w3id.org/ecsel-dr-SO#hasEventCalendarType> <http://www.w3.org/2000/01/rdf-schema#label> "has event calendar type"@en .
<http://www.w3id.org/ecsel-dr-SO#hasEventCalendarType> <http://www.w3.org/2000/01/rdf-schema#comment> "Event Calendar: Type of event"@en .
<http://www.w3id.org/ecsel-dr-SO#hasEventCalendarType> <http://www.w3.org/2000/01/rdf-schema#range> <http://www.w3.org/2001/XMLSchema#string> .
<http://www.w3id.org/ecsel-dr-SO#hasEventCalendarType> <http://www.w3.org/2000/01/rdf-schema#domain> <http://www.purl.org/i4go/variant-domain/operation/EventCalendar> .
<http://www.w3id.org/ecsel-dr-SO#hasEventCalendarType> <http://www.w3.org/2000/01/rdf-schema#subPropertyOf> <http://www.w3.org/2002/07/owl#topDataProperty> .
<http://www.w3id.org/ecsel-dr-SO#hasEventCalendarType> <http://www.w3.org/1999/02/22-rdf-syntax-ns#type> <http://www.w3.org/2002/07/owl#DatatypeProperty> .
<http://www.w3id.org/ecsel-dr-SO#hasScrappingProbabilityWafers> <http://www.w3.org/2000/01/rdf-schema#label> "has scrapping probability wafers"@en .
<http://www.w3id.org/ecsel-dr-SO#hasScrappingProbabilityWafers> <http://www.w3.org/2000/01/rdf-schema#comment> "Operation: Probability of scrapping-tested wafers to be scrapped."@en .
<http://www.w3id.org/ecsel-dr-SO#hasScrappingProbabilityWafers> <http://www.w3.org/2000/01/rdf-schema#range> <http://www.w3.org/2001/XMLSchema#double> .
<http://www.w3id.org/ecsel-dr-SO#hasScrappingProbabilityWafers> <http://www.w3.org/2000/01/rdf-schema#domain> <http://www.w3id.org/ecsel-dr-SO#Operation> .
<http://www.w3id.org/ecsel-dr-SO#hasScrappingProbabilityWafers> <http://www.w3.org/2000/01/rdf-schema#subPropertyOf> <http://www.w3.org/2002/07/owl#topDataProperty> .
<http://www.w3id.org/ecsel-dr-SO#hasScrappingProbabilityWafers> <http://www.w3.org/1999/02/22-rdf-syntax-ns#type> <http://www.w3.org/2002/07/owl#DatatypeProperty> .
<http://www.w3id.org/ecsel-dr-SO#hasRoute> <http://www.w3.org/2000/01/rdf-schema#label> "has route"@en .
<http://www.w3id.org/ecsel-dr-SO#hasRoute> <http://www.w3.org/2000/01/rdf-schema#comment> "This property is used to relate operations with their routes and simulation routes."@en .
<http://www.w3id.org/ecsel-dr-SO#hasRoute> <http://www.w3.org/2000/01/rdf-schema#range> <http://www.w3id.org/ecsel-dr-SO#Route> .
<http://www.w3id.org/ecsel-dr-SO#hasRoute> <http://www.w3.org/2000/01/rdf-schema#range> <http://www.purl.org/i4go/variant-domain/operation/SimulationRoute> .
<http://www.w3id.org/ecsel-dr-SO#hasRoute> <http://www.w3.org/2000/01/rdf-schema#domain> <http://www.w3id.org/ecsel-dr-SO#Technology> .
<http://www.w3id.org/ecsel-dr-SO#hasRoute> <http://www.w3.org/2000/01/rdf-schema#domain> <http://www.w3id.org/ecsel-dr-SO#Operation> .
<http://www.w3id.org/ecsel-dr-SO#hasRoute> <http://www.w3.org/2000/01/rdf-schema#domain> <http://www.purl.org/i4go/variant-domain/operation/SimulationPart> .
<http://www.w3id.org/ecsel-dr-SO#hasRoute> <http://www.w3.org/2000/01/rdf-schema#subPropertyOf> <http://www.w3.org/2002/07/owl#topObjectProperty> .
<http://www.w3id.org/ecsel-dr-SO#hasRoute> <http://www.w3.org/1999/02/22-rdf-syntax-ns#type> <http://www.w3.org/2002/07/owl#ObjectProperty> .
<http://www.purl.org/i4go/variant-domain/operation/SaturationRegion> <http://www.w3.org/2000/01/rdf-schema#label> "Saturation region"@en .
<http://www.purl.org/i4go/variant-domain/operation/SaturationRegion> <http://www.w3.org/2000/01/rdf-schema#comment> "This is the region in which transistor tends to behave as a closed switch. The transistor has the effect of its collector and Emitter being shorted. The collector and Emitter currents are maximum in this mode of operation."@en .
<http://www.purl.org/i4go/variant-domain/operation/SaturationRegion> <http://www.w3.org/2000/01/rdf-schema#subClassOf> <http://www.purl.org/i4go/variant-domain/operation/On-StateRegion> .
<http://www.purl.org/i4go/variant-domain/operation/SaturationRegion> <http://www.w3.org/1999/02/22-rdf-syntax-ns#type> <http://www.w3.org/2002/07/owl#Class> .
<http://www.purl.org/i4go/variant-domain/operation/ChemicalPolishing> <http://www.w3.org/2000/01/rdf-schema#label> "Chemical polishing"@en .
<http://www.purl.org/i4go/variant-domain/operation/ChemicalPolishing> <http://www.w3.org/2000/01/rdf-schema#comment> "The chemical polishing process or chemical mechanical planarization (CMP) is a process whereby a chemical reaction increases the mechanical removal rate of a material. CMP is commonly used to polish off high spots on wafers or films deposited on wafers, flattening the film or wafer, referred to as planarization. The chemical reaction that increases the mechanical removal rate is commonly tailored to provide a higher removal rate of one material versus another material. The chemical action in CMP helps to achieve higher selectivity's of one material to another than a strictly mechanical process would provide."@en .
<http://www.purl.org/i4go/variant-domain/operation/ChemicalPolishing> <http://www.w3.org/2000/01/rdf-schema#subClassOf> <http://www.w3id.org/ecsel-dr-SO#Workshop> .
<http://www.purl.org/i4go/variant-domain/operation/ChemicalPolishing> <http://www.w3.org/1999/02/22-rdf-syntax-ns#type> <http://www.w3.org/2002/07/owl#Class> .
<http://www.w3id.org/ecsel-dr-SO#hasEventCalendar> <http://www.w3.org/2000/01/rdf-schema#label> "has event calendar"@en .
<http://www.w3id.org/ecsel-dr-SO#hasEventCalendar> <http://www.w3.org/2000/01/rdf-schema#comment> "This property is used to relate operations with their event calendar."@en .
<http://www.w3id.org/ecsel-dr-SO#hasEventCalendar> <http://www.w3.org/2000/01/rdf-schema#range> <http://www.purl.org/i4go/variant-domain/operation/EventCalendar> .
<http://www.w3id.org/ecsel-dr-SO#hasEventCalendar> <http://www.w3.org/2000/01/rdf-schema#domain> <http://www.w3id.org/ecsel-dr-SO#Operation> .
<http://www.w3id.org/ecsel-dr-SO#hasEventCalendar> <http://www.w3.org/2000/01/rdf-schema#subPropertyOf> <http://www.w3.org/2002/07/owl#topObjectProperty> .
<http://www.w3id.org/ecsel-dr-SO#hasEventCalendar> <http://www.w3.org/1999/02/22-rdf-syntax-ns#type> <http://www.w3.org/2002/07/owl#ObjectProperty> .
_:A6b5d418bX3aX17a61612d50X3aXX2dX7ff6 <http://www.w3.org/2002/07/owl#unionOf> _:A6b5d418bX3aX17a61612d50X3aXX2dX7ff5 .
_:A6b5d418bX3aX17a61612d50X3aXX2dX7ff6 <http://www.w3.org/1999/02/22-rdf-syntax-ns#type> <http://www.w3.org/2002/07/owl#Class> .
_:A6b5d418bX3aX17a61612d50X3aXX2dX7fef <http://www.w3.org/1999/02/22-rdf-syntax-ns#rest> _:A6b5d418bX3aX17a61612d50X3aXX2dX7fee .
_:A6b5d418bX3aX17a61612d50X3aXX2dX7fef <http://www.w3.org/1999/02/22-rdf-syntax-ns#first> <http://www.w3id.org/ecsel-dr-SO#CurrentWIP> .
<http://www.w3id.org/ecsel-dr-SO#Diffusion> <http://www.w3.org/2000/01/rdf-schema#label> "Diffusion"@en .
<http://www.w3id.org/ecsel-dr-SO#Diffusion> <http://www.w3.org/2000/01/rdf-schema#comment> "Diffusion is a process whereby a substance redistributes from an area of relatively high concentration to an area of relatively low concentration due to random thermal motion. The larger the concentration gradient the faster diffusion occurs for a given temperature, conversely, the higher the temperature the faster diffusion occurs for a given concentration gradient."@en .
<http://www.w3id.org/ecsel-dr-SO#Diffusion> <http://www.w3.org/2000/01/rdf-schema#subClassOf> <http://www.w3id.org/ecsel-dr-SO#Workshop> .
<http://www.w3id.org/ecsel-dr-SO#Diffusion> <http://www.w3.org/1999/02/22-rdf-syntax-ns#type> <http://www.w3.org/2002/07/owl#Class> .
<http://www.w3id.org/ecsel-dr-SO#hasReworkOperation> <http://www.w3.org/2000/01/rdf-schema#label> "has rework operation"@en .
<http://www.w3id.org/ecsel-dr-SO#hasReworkOperation> <http://www.w3.org/2000/01/rdf-schema#comment> "Rework Operation, if needed."@en .
<http://www.w3id.org/ecsel-dr-SO#hasReworkOperation> <http://www.w3.org/2000/01/rdf-schema#range> <http://www.w3.org/2001/XMLSchema#string> .
<http://www.w3id.org/ecsel-dr-SO#hasReworkOperation> <http://www.w3.org/2000/01/rdf-schema#domain> <http://www.w3id.org/ecsel-dr-SO#Operation> .
<http://www.w3id.org/ecsel-dr-SO#hasReworkOperation> <http://www.w3.org/2000/01/rdf-schema#subPropertyOf> <http://www.w3.org/2002/07/owl#topDataProperty> .
<http://www.w3id.org/ecsel-dr-SO#hasReworkOperation> <http://www.w3.org/1999/02/22-rdf-syntax-ns#type> <http://www.w3.org/2002/07/owl#DatatypeProperty> .
<http://www.w3id.org/ecsel-dr-SO#hasMeanTimeToRepair> <http://www.w3.org/2000/01/rdf-schema#label> "has mean time to repair"@en .
<http://www.w3id.org/ecsel-dr-SO#hasMeanTimeToRepair> <http://www.w3.org/2000/01/rdf-schema#comment> "length of, or element of the length of, a temporal extent expressed in seconds"@en .
<http://www.w3id.org/ecsel-dr-SO#hasMeanTimeToRepair> <http://www.w3.org/2000/01/rdf-schema#range> <http://www.w3.org/2001/XMLSchema#double> .
<http://www.w3id.org/ecsel-dr-SO#hasMeanTimeToRepair> <http://www.w3.org/2000/01/rdf-schema#domain> <http://www.purl.org/i4go/variant-domain/operation/EventCalendar> .
<http://www.w3id.org/ecsel-dr-SO#hasMeanTimeToRepair> <http://www.w3.org/2000/01/rdf-schema#subPropertyOf> <http://www.w3.org/2002/07/owl#topDataProperty> .
<http://www.w3id.org/ecsel-dr-SO#hasMeanTimeToRepair> <http://www.w3.org/1999/02/22-rdf-syntax-ns#type> <http://www.w3.org/2002/07/owl#DatatypeProperty> .
_:A6b5d418bX3aX17a61612d50X3aXX2dX7ff0 <http://www.w3.org/1999/02/22-rdf-syntax-ns#rest> _:A6b5d418bX3aX17a61612d50X3aXX2dX7fef .
_:A6b5d418bX3aX17a61612d50X3aXX2dX7ff0 <http://www.w3.org/1999/02/22-rdf-syntax-ns#first> <http://www.purl.org/i4go/variant-domain/operation/EventCalendar> .
<http://www.w3id.org/ecsel-dr-SO#hasOperationCritical> <http://www.w3.org/2000/01/rdf-schema#label> "has operation critical"@en .
<http://www.w3id.org/ecsel-dr-SO#hasOperationCritical> <http://www.w3.org/2000/01/rdf-schema#comment> "Operation: Is the Operation critical in terms of SC planning (a Bottleneck) or not?"@en .
<http://www.w3id.org/ecsel-dr-SO#hasOperationCritical> <http://www.w3.org/2000/01/rdf-schema#range> <http://www.w3.org/2001/XMLSchema#boolean> .
<http://www.w3id.org/ecsel-dr-SO#hasOperationCritical> <http://www.w3.org/2000/01/rdf-schema#domain> <http://www.w3id.org/ecsel-dr-SO#Operation> .
<http://www.w3id.org/ecsel-dr-SO#hasOperationCritical> <http://www.w3.org/2000/01/rdf-schema#subPropertyOf> <http://www.w3.org/2002/07/owl#topDataProperty> .
<http://www.w3id.org/ecsel-dr-SO#hasOperationCritical> <http://www.w3.org/1999/02/22-rdf-syntax-ns#type> <http://www.w3.org/2002/07/owl#DatatypeProperty> .
<http://www.w3id.org/ecsel-dr-SO#hasReworkProbabilityWafers> <http://www.w3.org/2000/01/rdf-schema#label> "has rework probability wafers"@en .
<http://www.w3id.org/ecsel-dr-SO#hasReworkProbabilityWafers> <http://www.w3.org/2000/01/rdf-schema#comment> "Operation: Probability of rework-tested wafers to be reworked."@en .
<http://www.w3id.org/ecsel-dr-SO#hasReworkProbabilityWafers> <http://www.w3.org/2000/01/rdf-schema#range> <http://www.w3.org/2001/XMLSchema#double> .
<http://www.w3id.org/ecsel-dr-SO#hasReworkProbabilityWafers> <http://www.w3.org/2000/01/rdf-schema#domain> <http://www.w3id.org/ecsel-dr-SO#Operation> .
<http://www.w3id.org/ecsel-dr-SO#hasReworkProbabilityWafers> <http://www.w3.org/2000/01/rdf-schema#subPropertyOf> <http://www.w3.org/2002/07/owl#topDataProperty> .
<http://www.w3id.org/ecsel-dr-SO#hasReworkProbabilityWafers> <http://www.w3.org/1999/02/22-rdf-syntax-ns#type> <http://www.w3.org/2002/07/owl#DatatypeProperty> .
_:A6b5d418bX3aX17a61612d50X3aXX2dX7ffc <http://www.w3.org/2002/07/owl#unionOf> _:A6b5d418bX3aX17a61612d50X3aXX2dX7ffb .
_:A6b5d418bX3aX17a61612d50X3aXX2dX7ffc <http://www.w3.org/1999/02/22-rdf-syntax-ns#type> <http://www.w3.org/2002/07/owl#Class> .
<http://www.w3.org/ns/ssn/systems/OperatingRange> <http://www.w3.org/2000/01/rdf-schema#label> "Operating range"@en .
<http://www.w3.org/ns/ssn/systems/OperatingRange> <http://www.w3.org/2000/01/rdf-schema#comment> "Describes normal OperatingProperties of a System under some specified Conditions. For example, to the power requirement or maintenance schedule of a System under a specified temperature range.\nIn the absence of OperatingProperties, it simply describes the Conditions in which a System is expected to operate."@en .
<http://www.w3.org/ns/ssn/systems/OperatingRange> <http://www.w3.org/2000/01/rdf-schema#subClassOf> <http://www.w3.org/ns/ssn/Property> .
<http://www.w3.org/ns/ssn/systems/OperatingRange> <http://www.w3.org/1999/02/22-rdf-syntax-ns#type> <http://www.w3.org/2002/07/owl#Class> .
<http://www.w3id.org/ecsel-dr-SO#hasSplitLots> <http://www.w3.org/2000/01/rdf-schema#label> "has split lots"@en .
<http://www.w3id.org/ecsel-dr-SO#hasSplitLots> <http://www.w3.org/2000/01/rdf-schema#comment> "Split into # lots, added due to data import"@en .
<http://www.w3id.org/ecsel-dr-SO#hasSplitLots> <http://www.w3.org/2000/01/rdf-schema#range> <http://www.w3.org/2001/XMLSchema#integer> .
<http://www.w3id.org/ecsel-dr-SO#hasSplitLots> <http://www.w3.org/2000/01/rdf-schema#domain> <http://www.w3id.org/ecsel-dr-SO#Operation> .
<http://www.w3id.org/ecsel-dr-SO#hasSplitLots> <http://www.w3.org/2000/01/rdf-schema#subPropertyOf> <http://www.w3.org/2002/07/owl#topDataProperty> .
<http://www.w3id.org/ecsel-dr-SO#hasSplitLots> <http://www.w3.org/1999/02/22-rdf-syntax-ns#type> <http://www.w3.org/2002/07/owl#DatatypeProperty> .
<http://www.w3id.org/ecsel-dr-SO#Implantation> <http://www.w3.org/2000/01/rdf-schema#label> "Implantation"@en .
<http://www.w3id.org/ecsel-dr-SO#Implantation> <http://www.w3.org/2000/01/rdf-schema#comment> "Implantation or Ion Implantation is a technique where ions are accelerated to a higher energy and speed an injected into a semiconductor. The dominant techniques for introducing dopants into a semiconductor."@en .
<http://www.w3id.org/ecsel-dr-SO#Implantation> <http://www.w3.org/2000/01/rdf-schema#subClassOf> <http://www.w3id.org/ecsel-dr-SO#Workshop> .
<http://www.w3id.org/ecsel-dr-SO#Implantation> <http://www.w3.org/1999/02/22-rdf-syntax-ns#type> <http://www.w3.org/2002/07/owl#Class> .
<http://www.w3id.org/ecsel-dr-SO#isEquipmentOf> <http://www.w3.org/2000/01/rdf-schema#label> "is equipment of"@en .
<http://www.w3id.org/ecsel-dr-SO#isEquipmentOf> <http://www.w3.org/2000/01/rdf-schema#subPropertyOf> <http://www.w3.org/2002/07/owl#topObjectProperty> .
<http://www.w3id.org/ecsel-dr-SO#isEquipmentOf> <http://www.w3.org/1999/02/22-rdf-syntax-ns#type> <http://www.w3.org/2002/07/owl#ObjectProperty> .
<http://www.w3id.org/ecsel-dr-SO#hasDemand> <http://www.w3.org/2000/01/rdf-schema#label> "has demand"@en .
<http://www.w3id.org/ecsel-dr-SO#hasDemand> <http://www.w3.org/2000/01/rdf-schema#comment> "This property is used to relate operations with redundant demands and production requests."@en .
<http://www.w3id.org/ecsel-dr-SO#hasDemand> <http://www.w3.org/2000/01/rdf-schema#range> <http://www.purl.org/i4go/variant-domain/operation/ProductionRequests> .
<http://www.w3id.org/ecsel-dr-SO#hasDemand> <http://www.w3.org/2000/01/rdf-schema#range> <http://www.purl.org/i4go/variant-domain/operation/DemandSnapshot> .
<http://www.w3id.org/ecsel-dr-SO#hasDemand> <http://www.w3.org/2000/01/rdf-schema#domain> <http://www.w3id.org/ecsel-dr-SO#Operation> .
<http://www.w3id.org/ecsel-dr-SO#hasDemand> <http://www.w3.org/2000/01/rdf-schema#subPropertyOf> <http://www.w3.org/2002/07/owl#topObjectProperty> .
<http://www.w3id.org/ecsel-dr-SO#hasDemand> <http://www.w3.org/1999/02/22-rdf-syntax-ns#type> <http://www.w3.org/2002/07/owl#ObjectProperty> .
<http://www.purl.org/i4go/variant-domain/operation/SimulationPart> <http://www.w3.org/2000/01/rdf-schema#label> "Simulation part"@en .
<http://www.purl.org/i4go/variant-domain/operation/SimulationPart> <http://www.w3.org/2000/01/rdf-schema#comment> "A simulation part helps to identify the same product in different locations. They are visible in Product Structures. This is a simulation entity and not a form of production/planning."@en .
<http://www.purl.org/i4go/variant-domain/operation/SimulationPart> <http://www.w3.org/1999/02/22-rdf-syntax-ns#type> <http://www.w3.org/2002/07/owl#Class> .
<http://www.w3id.org/ecsel-dr-SO#hasVariancePTime> <http://www.w3.org/2000/01/rdf-schema#label> "has variance p time"@en .
<http://www.w3id.org/ecsel-dr-SO#hasVariancePTime> <http://www.w3.org/2000/01/rdf-schema#comment> "Length of, or element of the length of, a temporal extent expressed in seconds"@en .
<http://www.w3id.org/ecsel-dr-SO#hasVariancePTime> <http://www.w3.org/2000/01/rdf-schema#range> <http://www.w3.org/2001/XMLSchema#decimal> .
<http://www.w3id.org/ecsel-dr-SO#hasVariancePTime> <http://www.w3.org/2000/01/rdf-schema#domain> <http://www.w3id.org/ecsel-dr-SO#Operation> .
<http://www.w3id.org/ecsel-dr-SO#hasVariancePTime> <http://www.w3.org/2000/01/rdf-schema#subPropertyOf> <http://www.w3.org/2002/07/owl#topDataProperty> .
<http://www.w3id.org/ecsel-dr-SO#hasVariancePTime> <http://www.w3.org/1999/02/22-rdf-syntax-ns#type> <http://www.w3.org/2002/07/owl#DatatypeProperty> .
<http://www.w3id.org/ecsel-dr-SO#Operation> <http://www.w3.org/2000/01/rdf-schema#label> "Operation"@en .
<http://www.w3id.org/ecsel-dr-SO#Operation> <http://www.w3.org/2000/01/rdf-schema#comment> "The master entity \u201COperation\u201D depicts the generic behavior of a single process step. Each operation has a foreign key relation to equipment and to route which means that the operation is required by the specific routes and requires a specific equipment. (workflow descriptive master entity)."@en .
<http://www.w3id.org/ecsel-dr-SO#Operation> <http://www.w3.org/1999/02/22-rdf-syntax-ns#type> <http://www.w3.org/2002/07/owl#Class> .
<http://www.purl.org/i4go/variant-domain/operation/RegionOfOperation> <http://www.w3.org/2000/01/rdf-schema#label> "Region of operation"@en .
<http://www.purl.org/i4go/variant-domain/operation/RegionOfOperation> <http://www.w3.org/2000/01/rdf-schema#comment> "The supply of suitable external dc voltage is called as biasing. Either forward or reverse biasing is done to the emitter and collector junctions of the transistor. These biasing methods make the transistor circuit to work in four kinds of regions such as Active region, Saturation region, Cutoff region and Inverse active region."@en .
<http://www.purl.org/i4go/variant-domain/operation/RegionOfOperation> <http://www.w3.org/2000/01/rdf-schema#subClassOf> <http://www.purl.org/i4go/variant-domain/operation/OperatingProperty> .
<http://www.purl.org/i4go/variant-domain/operation/RegionOfOperation> <http://www.w3.org/1999/02/22-rdf-syntax-ns#type> <http://www.w3.org/2002/07/owl#Class> .
<http://www.w3id.org/ecsel-dr-SO#hasLotSize> <http://www.w3.org/2000/01/rdf-schema#label> "has lot size"@en .
<http://www.w3id.org/ecsel-dr-SO#hasLotSize> <http://www.w3.org/2000/01/rdf-schema#comment> "This property is used to relate operations with their lot size"@en .
<http://www.w3id.org/ecsel-dr-SO#hasLotSize> <http://www.w3.org/2000/01/rdf-schema#domain> _:A6b5d418bX3aX17a61612d50X3aXX2dX7ff6 .
<http://www.w3id.org/ecsel-dr-SO#hasLotSize> <http://www.w3.org/2000/01/rdf-schema#subPropertyOf> <http://www.w3.org/2002/07/owl#topObjectProperty> .
<http://www.w3id.org/ecsel-dr-SO#hasLotSize> <http://www.w3.org/1999/02/22-rdf-syntax-ns#type> <http://www.w3.org/2002/07/owl#ObjectProperty> .
<http://www.w3id.org/ecsel-dr-SO#hasTechnology> <http://www.w3.org/2000/01/rdf-schema#label> "has technology"@en .
<http://www.w3id.org/ecsel-dr-SO#hasTechnology> <http://www.w3.org/2000/01/rdf-schema#label> "This property is used to relate operations with their associated equipment and technologies."@en .
<http://www.w3id.org/ecsel-dr-SO#hasTechnology> <http://www.w3.org/2000/01/rdf-schema#range> <http://www.w3id.org/ecsel-dr-SO#Technology> .
<http://www.w3id.org/ecsel-dr-SO#hasTechnology> <http://www.w3.org/2000/01/rdf-schema#domain> <http://www.w3id.org/ecsel-dr-SO#Operation> .
<http://www.w3id.org/ecsel-dr-SO#hasTechnology> <http://www.w3.org/2000/01/rdf-schema#subPropertyOf> <http://www.w3.org/2002/07/owl#topObjectProperty> .
<http://www.w3id.org/ecsel-dr-SO#hasTechnology> <http://www.w3.org/1999/02/22-rdf-syntax-ns#type> <http://www.w3.org/2002/07/owl#ObjectProperty> .
<http://www.w3id.org/ecsel-dr-SO#hasTechnologyID> <http://www.w3.org/2000/01/rdf-schema#label> "has technology"@en .
<http://www.w3id.org/ecsel-dr-SO#hasTechnologyID> <http://www.w3.org/2000/01/rdf-schema#comment> "Name of the technology"@en .
<http://www.w3id.org/ecsel-dr-SO#hasTechnologyID> <http://www.w3.org/2000/01/rdf-schema#subPropertyOf> <http://www.w3.org/2002/07/owl#topDataProperty> .
<http://www.w3id.org/ecsel-dr-SO#hasTechnologyID> <http://www.w3.org/1999/02/22-rdf-syntax-ns#type> <http://www.w3.org/2002/07/owl#DatatypeProperty> .
_:A6b5d418bX3aX17a61612d50X3aXX2dX7ff5 <http://www.w3.org/1999/02/22-rdf-syntax-ns#rest> _:A6b5d418bX3aX17a61612d50X3aXX2dX7ff4 .
_:A6b5d418bX3aX17a61612d50X3aXX2dX7ff5 <http://www.w3.org/1999/02/22-rdf-syntax-ns#first> <http://www.purl.org/i4go/variant-domain/operation/EventCalendar> .
<http://www.w3id.org/ecsel-dr-SO#hasLotSizeQuantity> <http://www.w3.org/2000/01/rdf-schema#label> "has lot size quantity"@en .
<http://www.w3id.org/ecsel-dr-SO#hasLotSizeQuantity> <http://www.w3.org/2000/01/rdf-schema#comment> "Lot Size: Standard (FE) or optimal (BE) lot size for respective PL3"@en .
<http://www.w3id.org/ecsel-dr-SO#hasLotSizeQuantity> <http://www.w3.org/2000/01/rdf-schema#subPropertyOf> <http://www.w3.org/2002/07/owl#topDataProperty> .
<http://www.w3id.org/ecsel-dr-SO#hasLotSizeQuantity> <http://www.w3.org/1999/02/22-rdf-syntax-ns#type> <http://www.w3.org/2002/07/owl#DatatypeProperty> .
<http://www.w3id.org/ecsel-dr-SO#Workshop> <http://www.w3.org/2000/01/rdf-schema#label> "Workshop"@en .
<http://www.w3id.org/ecsel-dr-SO#Workshop> <http://www.w3.org/2000/01/rdf-schema#comment> "The overall organizational working structures within the fabs is described in the entity \u201CWorkshop\u201D."@en .
<http://www.w3id.org/ecsel-dr-SO#Workshop> <http://www.w3.org/1999/02/22-rdf-syntax-ns#type> <http://www.w3.org/2002/07/owl#Class> .
_:A6b5d418bX3aX17a61612d50X3aXX2dX7fee <http://www.w3.org/1999/02/22-rdf-syntax-ns#rest> <http://www.w3.org/1999/02/22-rdf-syntax-ns#nil> .
_:A6b5d418bX3aX17a61612d50X3aXX2dX7fee <http://www.w3.org/1999/02/22-rdf-syntax-ns#first> <http://www.w3id.org/ecsel-dr-SO#Operation> .
