@prefix :        <http://www.purl.org/i40go/variant-domain/manufacturingresource#> .
@prefix owl:     <http://www.w3.org/2002/07/owl#> .
@prefix rdf:     <http://www.w3.org/1999/02/22-rdf-syntax-ns#> .
@prefix terms:   <http://purl.org/dc/terms/> .
@prefix ns:      <http://creativecommons.org/ns#> .
@prefix xsd:     <http://www.w3.org/2001/XMLSchema#> .
@prefix rdfs:    <http://www.w3.org/2000/01/rdf-schema#> .
@prefix dc:      <http://purl.org/dc/elements/1.1/> .

<http://www.owl-ontologies.com/mason.owl#Resource>
      a       owl:Class ;
      rdfs:comment "Any capability that is to be scheduled, assigned or controlled by the underlying implementation to assure non-conflicting usage by processes."@en ;
      rdfs:label "Resource"@en ;
      rdfs:subClassOf <http://www.purl.org/i40go/common-domain/manufacture/ManufacturingConcept> .

<http://www.owl-ontologies.com/mason.owl#Building>
      a       owl:Class ;
      rdfs:subClassOf <http://www.purl.org/i40go/variant-domain/manufacturingresource/GeographicResource> .

<http://www.purl.org/i40go/variant-domain/manufacturingresource/ProgrammingOperator>
      a       owl:Class ;
      rdfs:label "Programming operator"@en ;
      rdfs:subClassOf <http://www.purl.org/i40go/variant-domain/manufacturingresource/HumanResource> .

<http://www.purl.org/i40go/variant-domain/manufacturingresource/ProceduresExpert>
      a       owl:Class ;
      rdfs:label "Procedures expert"@en ;
      rdfs:subClassOf <http://www.purl.org/i40go/variant-domain/manufacturingresource/HumanResource> .

<http://www.owl-ontologies.com/mason.owl#Operator>
      a       owl:Class ;
      rdfs:label "Operator"@en ;
      rdfs:subClassOf <http://www.purl.org/i40go/variant-domain/manufacturingresource/HumanResource> .

dc:title
      a       owl:AnnotationProperty .

<http://www.purl.org/i40go/variant-domain/manufacturingresource/MaterialResource>
      a       owl:Class ;
      rdfs:comment "Material resources are materials found in the natural world that have practical use and value for humans. Material resources include wood, glass (which comes from sand), metals, edible plants, and plastics (which are made from natural chemicals)."@en ;
      rdfs:label "Material resource"@en ;
      rdfs:subClassOf <http://www.owl-ontologies.com/mason.owl#Resource> .

<http://www.purl.org/i40go/variant-domain/manufacturingresource/GeographicResource>
      a       owl:Class ;
      rdfs:comment "A gepgraphic resource is any physical material constituting part of Earth that people need and value."@en ;
      rdfs:label "Geographic resource"@en ;
      rdfs:subClassOf <http://www.owl-ontologies.com/mason.owl#Resource> .

ns:license
      a       owl:AnnotationProperty .

<http://www.purl.org/i40go/variant-domain/manufacturingresource/HumanResource>
      a       owl:Class ;
      rdfs:comment "The personnel of a business or organization, regarded as a significant asset in terms of skills and abilities."@en ;
      rdfs:label "Human resource"@en ;
      rdfs:subClassOf <http://www.owl-ontologies.com/mason.owl#Resource> .

<http://www.purl.org/i40go/variant-domain/manufacturingresource/BuildingZone>
      a       owl:Class ;
      rdfs:comment "Each zone determines a building's shape and permitted uses. A building's shape is controlled by zonal restrictions on allowable floor area ratio and height (in absolute terms and in relation with adjacent buildings and roads)."@en ;
      rdfs:label "Building zone"@en ;
      rdfs:subClassOf <http://www.purl.org/i40go/variant-domain/manufacturingresource/GeographicResource> .

<http://www.purl.org/i40go/variant-domain/manufacturingresource/PreparationOperator>
      a       owl:Class ;
      rdfs:label "Preparation operator"@en ;
      rdfs:subClassOf <http://www.purl.org/i40go/variant-domain/manufacturingresource/HumanResource> .

<http://www.owl-ontologies.com/mason.owl#Site>
      a       owl:Class ;
      rdfs:comment "An area of ground on which a town, building, or monument is constructed."@en ;
      rdfs:label "Site"@en ;
      rdfs:subClassOf <http://www.purl.org/i40go/variant-domain/manufacturingresource/GeographicResource> .

<http://www.purl.org/i40go/variant-domain/manufacturingresource>
      a       owl:Ontology ;
      rdfs:comment "The 'Manufacturing Resource' ontology module represents data about the resources (i.e., tools, human resources) used during the manufacturing process."@en ;
      ns:license "https://creativecommons.org/licenses/by-nc/4.0/"@en ;
      dc:title "Manufacturing Resource ontology"@en ;
      terms:creator """Javier Cuenca <mailto:jcuenca@mondragon.edu>
Felix Larrinaga <mailto:flarrinaga@mondragon.edu>"""@en ;
      terms:issued "2021-24-05"@en ;
      owl:imports <http://www.purl.org/i40go/common-domain/manufacture> ;
      owl:versionInfo "1.0"@en .

terms:issued
      a       owl:AnnotationProperty .

terms:creator
      a       owl:AnnotationProperty .

<http://www.owl-ontologies.com/mason.owl#HandlingOperator>
      a       owl:Class ;
      rdfs:label "Handling operator"@en ;
      rdfs:subClassOf <http://www.purl.org/i40go/variant-domain/manufacturingresource/HumanResource> .
